@prefix : <https://w3id.org/ontouml/2.0.0#> .
@prefix dct: <http://purl.org/dc/terms/> .
@prefix owl: <http://www.w3.org/2002/07/owl#> .
@prefix rdf: <http://www.w3.org/1999/02/22-rdf-syntax-ns#> .
@prefix xml: <http://www.w3.org/XML/1998/namespace> .
@prefix xsd: <http://www.w3.org/2001/XMLSchema#> .
@prefix dcat: <http://www.w3.org/ns/dcat#> .
@prefix foaf: <http://xmlns.com/foaf/0.1/> .
@prefix rdfs: <http://www.w3.org/2000/01/rdf-schema#> .
@prefix vann: <http://purl.org/vocab/vann/> .
@prefix ontouml: <https://w3id.org/ontouml/2.0.0#> .
@base <https://w3id.org/ontouml/2.0.0> .

<https://w3id.org/ontouml/2.0.0> rdf:type owl:Ontology ;
                                  owl:versionIRI <https://w3id.org/ontouml/vocabulary/v2.0.0> ;
                                  dct:conformsTo <https://w3id.org/ontouml/metamodel/v2.0.0> ;
                                  dct:contributor <https://orcid.org/0000-0003-3385-4769> ;
                                  dct:creator <https://orcid.org/0000-0002-5385-5761> ,
                                              <https://orcid.org/0000-0003-2528-3118> ,
                                              <https://orcid.org/0000-0003-2736-7817> ;
                                  dct:description "An OWL vocabulary to allow the serialization and exchanging of OntoUML models in conformance with the Ontouml Metamodel."@en ;
                                  dct:identifier "https://w3id.org/ontouml"^^xsd:anyURI ;
                                  dct:isReferencedBy <https://dblp.org/rec/conf/jowo/FonsecaSVFGA21.html> ,
                                                     <https://doi.org/10.1007/978-3-031-17995-2_1> ;
                                  dct:issued "2022-04-03"^^xsd:date ;
                                  dct:language <http://id.loc.gov/vocabulary/iso639-1/en> ;
                                  dct:license <https://creativecommons.org/licenses/by-sa/4.0> ;
                                  dct:modified "2023-08-14"^^xsd:date ;
                                  dct:publisher <https://www.utwente.nl/en/eemcs/scs/> ;
                                  dct:title "OntoUML Vocabulary"@en ;
                                  vann:preferredNamespacePrefix "ontouml" ;
                                  vann:preferredNamespaceUri "https://w3id.org/ontouml#"^^xsd:anyURI ;
                                  owl:priorVersion <https://w3id.org/ontouml/vocabulary/v1.1.0> ;
                                  owl:versionInfo "Release compatible with the OntoUML Metamodel 2.0.0."@en ;
                                  dcat:keyword "OntoUML"@en ,
                                               "OntoUML Metamodel"@en ,
                                               "Ontology-Driven Conceptual Modeling"@en ;
                                  dcat:landingPage <https://w3id.org/ontouml/vocabulary> ;
                                  foaf:homepage <https://w3id.org/ontouml/vocabulary/docs> .

#################################################################
#    Annotation properties
#################################################################

###  http://purl.org/dc/terms/conformsTo
dct:conformsTo rdf:type owl:AnnotationProperty .


###  http://purl.org/dc/terms/contributor
dct:contributor rdf:type owl:AnnotationProperty .


###  http://purl.org/dc/terms/creator
dct:creator rdf:type owl:AnnotationProperty .


###  http://purl.org/dc/terms/description
dct:description rdf:type owl:AnnotationProperty .


###  http://purl.org/dc/terms/identifier
dct:identifier rdf:type owl:AnnotationProperty .


###  http://purl.org/dc/terms/isReferencedBy
dct:isReferencedBy rdf:type owl:AnnotationProperty .


###  http://purl.org/dc/terms/issued
dct:issued rdf:type owl:AnnotationProperty .


###  http://purl.org/dc/terms/language
dct:language rdf:type owl:AnnotationProperty .


###  http://purl.org/dc/terms/license
dct:license rdf:type owl:AnnotationProperty .


###  http://purl.org/dc/terms/modified
dct:modified rdf:type owl:AnnotationProperty .


###  http://purl.org/dc/terms/publisher
dct:publisher rdf:type owl:AnnotationProperty .


###  http://purl.org/dc/terms/title
dct:title rdf:type owl:AnnotationProperty .


###  http://purl.org/vocab/vann/preferredNamespacePrefix
vann:preferredNamespacePrefix rdf:type owl:AnnotationProperty .


###  http://purl.org/vocab/vann/preferredNamespaceUri
vann:preferredNamespaceUri rdf:type owl:AnnotationProperty .


###  http://www.w3.org/ns/dcat#keyword
dcat:keyword rdf:type owl:AnnotationProperty .


###  http://www.w3.org/ns/dcat#landingPage
dcat:landingPage rdf:type owl:AnnotationProperty .


###  http://xmlns.com/foaf/0.1/homepage
foaf:homepage rdf:type owl:AnnotationProperty .


###  http://xmlns.com/foaf/0.1/mbox
foaf:mbox rdf:type owl:AnnotationProperty .


###  http://xmlns.com/foaf/0.1/member
foaf:member rdf:type owl:AnnotationProperty .


###  http://xmlns.com/foaf/0.1/name
foaf:name rdf:type owl:AnnotationProperty .


#################################################################
#    Datatypes
#################################################################

###  http://org.semanticweb.owlapi/error#Error3
<http://org.semanticweb.owlapi/error#Error3> rdf:type rdfs:Datatype .


###  http://org.semanticweb.owlapi/error#Error4
<http://org.semanticweb.owlapi/error#Error4> rdf:type rdfs:Datatype .


#################################################################
#    Object Properties
#################################################################

###  https://w3id.org/ontouml/2.0.0#aggregationKind
ontouml:aggregationKind rdf:type owl:ObjectProperty ;
                        rdfs:domain ontouml:Property ;
                        rdfs:range ontouml:AggregationKind ;
                        rdfs:comment "Characterizes an ontouml:Property with an ontouml:AggregationKind instance, i.e., indicates whether the ontouml:Property is a simple (ontouml:none), a shared (ontouml:shared), or a composite (ontouml:composite) property."@en ;
                        rdfs:isDefinedBy <https://w3id.org/ontouml/2.0.0> ;
                        rdfs:label "aggregation kind"@en .


###  https://w3id.org/ontouml/2.0.0#attribute
ontouml:attribute rdf:type owl:ObjectProperty ;
                  rdfs:subPropertyOf ontouml:property ;
                  rdfs:domain ontouml:Class ;
                  rdfs:range ontouml:Property ;
                  rdfs:comment "Relates an instance of an ontouml:Class to its properties, which are instances of the ontouml:Property class."@en ;
                  rdfs:isDefinedBy <https://w3id.org/ontouml/2.0.0> ;
                  rdfs:label "attribute"@en .


###  https://w3id.org/ontouml/2.0.0#cardinality
ontouml:cardinality rdf:type owl:ObjectProperty ;
                    rdfs:domain ontouml:Property ;
                    rdfs:range ontouml:Cardinality ;
                    rdfs:comment "Identifies the individual of type ontouml:Cardinality that represents the cardinalities of an ontouml:Property."@en ;
                    rdfs:isDefinedBy <https://w3id.org/ontouml/2.0.0> ;
                    rdfs:label "cardinality"@en .


###  https://w3id.org/ontouml/2.0.0#categorizer
ontouml:categorizer rdf:type owl:ObjectProperty ;
                    rdfs:domain ontouml:GeneralizationSet ;
                    rdfs:range ontouml:Class ;
                    rdfs:comment " Identifies the ontouml:Class that is instantiated by the specific classes of the ontouml:Generalization type composing the ontouml:GeneralizationSet"@en ;
                    rdfs:isDefinedBy <https://w3id.org/ontouml/2.0.0> ;
                    rdfs:label "categorizer"@en ;
                    rdfs:seeAlso <https://doi.org/10.1007/978-3-031-17995-2_2> ,
                                 <https://doi.org/10.1016/j.datak.2022.102012> .


###  https://w3id.org/ontouml/2.0.0#containsModelElement
ontouml:containsModelElement rdf:type owl:ObjectProperty ;
                             rdfs:domain ontouml:Package ;
                             rdfs:range ontouml:ModelElement ;
                             rdfs:comment "Identifies an instance of type ontouml:ModelElement that composes in an ontouml:Package."@en ,
                                          "It is mapped to the OntoUML Metamodel's 'contents' relation between the Package and ModelElement classes."@en ;
                             rdfs:isDefinedBy <https://w3id.org/ontouml/2.0.0> ;
                             rdfs:label "contains model element"@en .


###  https://w3id.org/ontouml/2.0.0#containsView
ontouml:containsView rdf:type owl:ObjectProperty ;
                     rdfs:domain ontouml:Diagram ;
                     rdfs:range ontouml:View ;
                     rdfs:comment "Identifies an instance of type ontouml:ElementView that is contained in an ontouml:Diagram, representing the concrete diagramation of an ontouml:ModelElement."@en ;
                     rdfs:isDefinedBy <https://w3id.org/ontouml/2.0.0> ;
                     rdfs:label "contains view"@en .


###  https://w3id.org/ontouml/2.0.0#diagram
ontouml:diagram rdf:type owl:ObjectProperty ;
                rdfs:domain ontouml:Project ;
                rdfs:range ontouml:Diagram ;
                rdfs:comment "Identifies which entities of type ontouml:Diagram are part of an ontouml:Project."@en ,
                             "It is mapped to the OntoUML Metamodel's 'diagrams' relation between the Project and Diagram classes."@en ;
                rdfs:isDefinedBy <https://w3id.org/ontouml/2.0.0> ;
                rdfs:label "diagram"@en .


###  https://w3id.org/ontouml/2.0.0#general
ontouml:general rdf:type owl:ObjectProperty ;
                rdfs:domain ontouml:Generalization ;
                rdfs:range ontouml:Classifier ;
                rdfs:comment "Identifies the parent ontouml:Classifier (e.g., a superclass) that participates in an ontouml:Generalization relation."@en ;
                rdfs:isDefinedBy <https://w3id.org/ontouml/2.0.0> ;
                rdfs:label "general"@en .


###  https://w3id.org/ontouml/2.0.0#generalization
ontouml:generalization rdf:type owl:ObjectProperty ;
                       rdfs:domain ontouml:GeneralizationSet ;
                       rdfs:range ontouml:Generalization ;
                       rdfs:comment "Identifies an ontouml:Generalization that participates in an ontouml:GeneralizationSet."@en ;
                       rdfs:isDefinedBy <https://w3id.org/ontouml/2.0.0> ;
                       rdfs:label "generalization"@en .


###  https://w3id.org/ontouml/2.0.0#isViewOf
ontouml:isViewOf rdf:type owl:ObjectProperty ;
                 rdfs:domain ontouml:View ;
                 rdfs:range ontouml:ModelElement ;
                 rdfs:comment "Relates an ontouml:ElementView to ontouml:ModelElement, indicating the diagrammatical representation of the latter in an ontouml:Diagram."@en ;
                 rdfs:isDefinedBy <https://w3id.org/ontouml/2.0.0> ;
                 rdfs:label "is view of"@en .


###  https://w3id.org/ontouml/2.0.0#literal
ontouml:literal rdf:type owl:ObjectProperty ;
                rdfs:domain ontouml:Class ;
                rdfs:range ontouml:Literal ;
                rdfs:comment "Relates an ontouml:Literal to its container enumeration class (an ontouml:Class that has the ontouml:stereotype property with ontouml:enumeration)."@en ;
                rdfs:isDefinedBy <https://w3id.org/ontouml/2.0.0> ;
                rdfs:label "literal"@en .


###  https://w3id.org/ontouml/2.0.0#model
ontouml:model rdf:type owl:ObjectProperty ;
              rdfs:domain ontouml:Project ;
              rdfs:range ontouml:Package ;
              rdfs:comment "Relates an ontouml:Project to an ontouml:Package that is part of it."@en ;
              rdfs:isDefinedBy <https://w3id.org/ontouml/2.0.0> ;
              rdfs:label "model"@en .


###  https://w3id.org/ontouml/2.0.0#owner
ontouml:owner rdf:type owl:ObjectProperty ;
              rdfs:domain ontouml:Diagram ;
              rdfs:range ontouml:ModelElement ;
              rdfs:comment "Relates an ontouml:Diagram to an ontouml:ModelElement that is represented on it, i.e., to an ontouml:ModelElement that has an ontouml:ElementView on that ontouml:Diagram."@en ;
              rdfs:isDefinedBy <https://w3id.org/ontouml/2.0.0> ;
              rdfs:label "owner"@en .


###  https://w3id.org/ontouml/2.0.0#point
ontouml:point rdf:type owl:ObjectProperty ;
              rdfs:domain ontouml:Path ;
              rdfs:range ontouml:Point ;
              rdfs:comment "Relates an ontouml:Path to an ontouml:Point that composes it."@en ;
              rdfs:isDefinedBy <https://w3id.org/ontouml/2.0.0> ;
              rdfs:label "point"@en .


###  https://w3id.org/ontouml/2.0.0#project
ontouml:project rdf:type owl:ObjectProperty ;
                rdfs:range ontouml:Project ;
                rdfs:comment "Relates an ontouml:OntoumlElement different than ontouml:Project to an ontouml:Project that it composes."@en ;
                rdfs:isDefinedBy <https://w3id.org/ontouml/2.0.0> ;
                rdfs:label "project"@en .


###  https://w3id.org/ontouml/2.0.0#property
ontouml:property rdf:type owl:ObjectProperty ;
                 rdfs:domain ontouml:Classifier ;
                 rdfs:range ontouml:Property ;
                 rdfs:comment "Aggregates its subproperties ontouml:attribute and ontouml:relationEnd. Should not be directly used."@en ,
                              "Identifies an ontouml:Property exhibited by an ontouml:Classifier. If the ontouml:Classifier is of type ontouml:Class, the ontouml:property is specialized in ontouml:attribute. If the ontouml:Classifier is an ontouml:Relation, the property is specialized in ontouml:relationEnd."@en ;
                 rdfs:isDefinedBy <https://w3id.org/ontouml/2.0.0> ;
                 rdfs:label "property"@en .


###  https://w3id.org/ontouml/2.0.0#propertyType
ontouml:propertyType rdf:type owl:ObjectProperty ;
                     rdfs:domain ontouml:Property ;
                     rdfs:range ontouml:Classifier ;
                     rdfs:comment "Identifies an ontouml:Class or ontouml:Relation (i.e., an ontouml:Classifier) to which an ontouml:Property refers."@en ;
                     rdfs:isDefinedBy <https://w3id.org/ontouml/2.0.0> ;
                     rdfs:label "property type"@en .


###  https://w3id.org/ontouml/2.0.0#redefinesProperty
ontouml:redefinesProperty rdf:type owl:ObjectProperty ;
                          rdfs:domain ontouml:Property ;
                          rdfs:range ontouml:Property ;
                          rdfs:comment "Identifies a target ontouml:Property that is redefined by a source ontouml:Property."@en ;
                          rdfs:isDefinedBy <https://w3id.org/ontouml/2.0.0> ;
                          rdfs:label "redefines property"@en .


###  https://w3id.org/ontouml/2.0.0#relationEnd
ontouml:relationEnd rdf:type owl:ObjectProperty ;
                    rdfs:subPropertyOf ontouml:property ;
                    rdfs:domain ontouml:Relation ;
                    rdfs:range ontouml:Property ;
                    rdfs:comment "Identifies a property that represents one end (source or target) of an ontouml:Relation."@en ;
                    rdfs:isDefinedBy <https://w3id.org/ontouml/2.0.0> ;
                    rdfs:label "relation end"@en .


###  https://w3id.org/ontouml/2.0.0#restrictedTo
ontouml:restrictedTo rdf:type owl:ObjectProperty ;
                     rdfs:domain ontouml:Class ;
                     rdfs:range ontouml:OntologicalNature ;
                     rdfs:comment "Associates an ontouml:Class to an ontouml:OntologicalNature, restricting its allowed values."@en ;
                     rdfs:isDefinedBy <https://w3id.org/ontouml/2.0.0> ;
                     rdfs:label "restricted to"@en .


###  https://w3id.org/ontouml/2.0.0#shape
ontouml:shape rdf:type owl:ObjectProperty ;
              rdfs:domain ontouml:View ;
              rdfs:range ontouml:Shape ;
              rdfs:comment "Relates an ontouml:ElementView to an ontouml:Shape that contains the diagramation's data (size and position) about the ontouml:ModelElement it is a view of."@en ;
              rdfs:isDefinedBy <https://w3id.org/ontouml/2.0.0> ;
              rdfs:label "shape"@en .


###  https://w3id.org/ontouml/2.0.0#sourceEnd
ontouml:sourceEnd rdf:type owl:ObjectProperty ;
                  rdfs:subPropertyOf ontouml:relationEnd ;
                  rdfs:domain ontouml:Relation ;
                  rdfs:range ontouml:Property ;
                  rdfs:comment "Identifies an ontouml:Property that represents the source side of an ontouml:Relation."@en ;
                  rdfs:isDefinedBy <https://w3id.org/ontouml/2.0.0> ;
                  rdfs:label "source end"@en .


###  https://w3id.org/ontouml/2.0.0#sourceView
ontouml:sourceView rdf:type owl:ObjectProperty ;
                   rdfs:domain ontouml:BinaryConnectorView ;
                   rdfs:range ontouml:View ;
                   rdfs:comment "Identifies an ontouml:ElementView that participates as source of an ontouml:RelationView or ontouml:GeneralizationView."@en ;
                   rdfs:isDefinedBy <https://w3id.org/ontouml/2.0.0> ;
                   rdfs:label "source view"@en .


###  https://w3id.org/ontouml/2.0.0#specific
ontouml:specific rdf:type owl:ObjectProperty ;
                 rdfs:domain ontouml:Generalization ;
                 rdfs:range ontouml:Classifier ;
                 rdfs:comment "Identifies the child ontouml:Classifier (e.g., a subclass) that participates in an ontouml:Generalization relation."@en ;
                 rdfs:isDefinedBy <https://w3id.org/ontouml/2.0.0> ;
                 rdfs:label "specific"@en .


###  https://w3id.org/ontouml/2.0.0#stereotype
ontouml:stereotype rdf:type owl:ObjectProperty ;
                   rdfs:domain ontouml:DecoratableElement ;
                   rdfs:range ontouml:Stereotype ;
                   rdfs:comment "Identifies the ontouml:Stereotype applied to the ontouml:DecoratableElement."@en ;
                   rdfs:isDefinedBy <https://w3id.org/ontouml/2.0.0> ;
                   rdfs:label "stereotype"@en .


###  https://w3id.org/ontouml/2.0.0#subsetsProperty
ontouml:subsetsProperty rdf:type owl:ObjectProperty ;
                        rdfs:domain ontouml:Property ;
                        rdfs:range ontouml:Property ;
                        rdfs:comment "Identifies a target ontouml:Property that is subsetted by a source ontouml:Property."@en ;
                        rdfs:isDefinedBy <https://w3id.org/ontouml/2.0.0> ;
                        rdfs:label "subsets property"@en .


###  https://w3id.org/ontouml/2.0.0#targetEnd
ontouml:targetEnd rdf:type owl:ObjectProperty ;
                  rdfs:subPropertyOf ontouml:relationEnd ;
                  rdfs:domain ontouml:Relation ;
                  rdfs:range ontouml:Property ;
                  rdfs:comment "Identifies an ontouml:Property that represents the target side of an ontouml:Relation."@en ;
                  rdfs:isDefinedBy <https://w3id.org/ontouml/2.0.0> ;
                  rdfs:label "target end"@en .


###  https://w3id.org/ontouml/2.0.0#targetView
ontouml:targetView rdf:type owl:ObjectProperty ;
                   rdfs:domain ontouml:BinaryConnectorView ;
                   rdfs:range ontouml:View ;
                   rdfs:comment "Identifies an ontouml:ElementView that participates as target of an ontouml:ConnectorView."@en ;
                   rdfs:isDefinedBy <https://w3id.org/ontouml/2.0.0> ;
                   rdfs:label "target view"@en .


###  https://w3id.org/ontouml/2.0.0#topLeftPosition
ontouml:topLeftPosition rdf:type owl:ObjectProperty ;
                        rdfs:domain ontouml:RectangularShape ;
                        rdfs:range ontouml:Point ;
                        rdfs:comment "Is direct mapped to the OntoUML Metamodel's 'topLeft' relationship between the classes RectangularShape and Point."@en ,
                                     "Relates an ontouml:RectangularShape to an ontouml:Point that contains the horizontal and vertical coordinates (ontouml:xCoordinate and ontouml:yCoordinate, respectively) representing the former's top left position in an ontouml:Diagram."@en ;
                        rdfs:isDefinedBy <https://w3id.org/ontouml/2.0.0> ;
                        rdfs:label "top left position"@en .


#################################################################
#    Data properties
#################################################################

###  https://w3id.org/ontouml/2.0.0#cardinalityValue
ontouml:cardinalityValue rdf:type owl:DatatypeProperty ;
                         rdfs:domain ontouml:Cardinality ;
                         rdfs:range xsd:string ;
                         rdfs:comment "Provides the complete (i.e., both lower and upper cardinality's bounds) cardinalities of an ontouml:Property via its related ontouml:Cardinality."@en ;
                         rdfs:isDefinedBy <https://w3id.org/ontouml/2.0.0> ;
                         rdfs:label "cardinality value"@en .


###  https://w3id.org/ontouml/2.0.0#description
ontouml:description rdf:type owl:DatatypeProperty ;
                    rdfs:domain ontouml:OntoumlElement ;
                    rdfs:range [ rdf:type rdfs:Datatype ;
                                 owl:unionOf ( <http://org.semanticweb.owlapi/error#Error4>
                                               xsd:string
                                             )
                               ] ;
                    rdfs:comment "Relates an ontouml:OntoumlElement to a string representing its description in free textual format."@en ;
                    rdfs:isDefinedBy <https://w3id.org/ontouml/2.0.0> ;
                    rdfs:label "description"@en .


###  https://w3id.org/ontouml/2.0.0#height
ontouml:height rdf:type owl:DatatypeProperty ;
               rdfs:domain ontouml:RectangularShape ;
               rdfs:range xsd:positiveInteger ;
               rdfs:comment "Indicates the height of an ontouml:RectangularShape that is represented in an ontouml:Diagram."@en ;
               rdfs:isDefinedBy <https://w3id.org/ontouml/2.0.0> ;
               rdfs:label "height"@en .


###  https://w3id.org/ontouml/2.0.0#isAbstract
ontouml:isAbstract rdf:type owl:DatatypeProperty ;
                   rdfs:domain ontouml:Classifier ;
                   rdfs:range xsd:boolean ;
                   rdfs:comment "Indicates if the ontouml:Classifier can have direct instances. If set to true, the classifier must be specialized before being instantiated. Otherwise, it can have direct instances."@en ;
                   rdfs:isDefinedBy <https://w3id.org/ontouml/2.0.0> ;
                   rdfs:label "is abstract"@en .


###  https://w3id.org/ontouml/2.0.0#isComplete
ontouml:isComplete rdf:type owl:DatatypeProperty ;
                   rdfs:domain ontouml:GeneralizationSet ;
                   rdfs:range xsd:boolean ;
                   rdfs:comment "Indicates if an ontouml:GeneralizationSet is complete, i.e., if it does not admit further generalizations."@en ;
                   rdfs:isDefinedBy <https://w3id.org/ontouml/2.0.0> ;
                   rdfs:label "is complete"@en .


###  https://w3id.org/ontouml/2.0.0#isDerived
ontouml:isDerived rdf:type owl:DatatypeProperty ;
                  rdfs:domain ontouml:DecoratableElement ;
                  rdfs:range xsd:boolean ;
                  rdfs:comment "Indicates if an ontouml:DecoratableElement can be defined through a derivation rule."@en ;
                  rdfs:isDefinedBy <https://w3id.org/ontouml/2.0.0> ;
                  rdfs:label "is derived"@en .


###  https://w3id.org/ontouml/2.0.0#isDisjoint
ontouml:isDisjoint rdf:type owl:DatatypeProperty ;
                   rdfs:domain ontouml:GeneralizationSet ;
                   rdfs:range xsd:boolean ;
                   rdfs:comment "Indicates if an ontouml:GeneralizationSet is disjoint, i.e., it does not admit generalizations having overlapping subclasses."@en ;
                   rdfs:isDefinedBy <https://w3id.org/ontouml/2.0.0> ;
                   rdfs:label "is disjoint"@en .


###  https://w3id.org/ontouml/2.0.0#isExtensional
ontouml:isExtensional rdf:type owl:DatatypeProperty ;
                      rdfs:domain ontouml:Class ;
                      rdfs:range xsd:boolean ;
                      rdfs:comment "Indicates if an ontouml:Class is extensionally defined (i.e., it's parts cannot change)."@en ;
                      rdfs:isDefinedBy <https://w3id.org/ontouml/2.0.0> ;
                      rdfs:label "is extensional"@en .


###  https://w3id.org/ontouml/2.0.0#isOrdered
ontouml:isOrdered rdf:type owl:DatatypeProperty ;
                  rdfs:domain ontouml:Property ;
                  rdfs:range xsd:boolean ;
                  rdfs:comment "Indicates if an ontouml:Property is ordered or not, i.e., if it requires an exact order of its values or not."@en ;
                  rdfs:isDefinedBy <https://w3id.org/ontouml/2.0.0> ;
                  rdfs:label "is ordered"@en .


###  https://w3id.org/ontouml/2.0.0#isPowertype
ontouml:isPowertype rdf:type owl:DatatypeProperty ;
                    rdfs:domain ontouml:Class ;
                    rdfs:range xsd:boolean ;
                    rdfs:comment "Indicates if an ontouml:Class is a powertype in multi-level modeling."@en ,
                                 "The ontouml:Class data property ontouml:isPowertype must not be true when it has an ontouml:order equal to one."@en ;
                    rdfs:isDefinedBy <https://w3id.org/ontouml/2.0.0> ;
                    rdfs:label "is powertype"@en ;
                    rdfs:seeAlso <https://doi.org/10.1007/978-3-031-17995-2_2> .


###  https://w3id.org/ontouml/2.0.0#isReadOnly
ontouml:isReadOnly rdf:type owl:DatatypeProperty ;
                   rdfs:domain ontouml:Property ;
                   rdfs:range xsd:boolean ;
                   rdfs:comment "Indicates if an ontouml:Property can or cannot be updated or modified."@en ;
                   rdfs:isDefinedBy <https://w3id.org/ontouml/2.0.0> ;
                   rdfs:label "is read only"@en .


###  https://w3id.org/ontouml/2.0.0#lowerBound
ontouml:lowerBound rdf:type owl:DatatypeProperty ;
                   rdfs:domain ontouml:Cardinality ;
                   rdfs:range xsd:nonNegativeInteger ;
                   rdfs:comment "An ontouml:Cardinality's lower bound must correspond to the one indicated by its ontouml:cardinalityValue property." ,
                                "E.g., if the ontouml:cardinalityValue set is [1..*] then the lower bound is '1'."@en ,
                                "Identifies the lower bound of an ontouml:Cardinality."@en ;
                   rdfs:isDefinedBy <https://w3id.org/ontouml/2.0.0> ;
                   rdfs:label "lower bound"@en .


###  https://w3id.org/ontouml/2.0.0#name
ontouml:name rdf:type owl:DatatypeProperty ;
             rdfs:domain ontouml:OntoumlElement ;
             rdfs:range [ rdf:type rdfs:Datatype ;
                          owl:unionOf ( <http://org.semanticweb.owlapi/error#Error3>
                                        xsd:string
                                      )
                        ] ;
             rdfs:comment "A string that identifies or names an ontouml:OntoumlElement."@en ;
             rdfs:isDefinedBy <https://w3id.org/ontouml/2.0.0> ;
             rdfs:label "name"@en .


###  https://w3id.org/ontouml/2.0.0#order
ontouml:order rdf:type owl:DatatypeProperty ;
              rdfs:domain ontouml:Class ;
              rdfs:range xsd:nonNegativeInteger ;
              rdfs:comment "Constraint: an ontouml:Class that has an ontouml:stereotype property with an ontouml:Stereotype different than ontouml:type must have an ontouml:order value equal to 1."@en ,
                           "Constraint: an ontouml:Class that has an ontouml:stereotype property with an ontouml:Stereotype ontouml:type must have an ontouml:order value grater than 1."@en ,
                           "Indicates the order of an ontouml:Class, enabling multi-level modeling."@en ;
              rdfs:isDefinedBy <https://w3id.org/ontouml/2.0.0> ;
              rdfs:label "order"@en ;
              rdfs:seeAlso <https://doi.org/10.1007/978-3-031-17995-2_2> .


###  https://w3id.org/ontouml/2.0.0#text
ontouml:text rdf:type owl:DatatypeProperty ;
             rdfs:domain ontouml:Note ;
             rdfs:range xsd:string ;
             rdfs:comment "A string that register any information of an ontouml:Note"@en ;
             rdfs:isDefinedBy <https://w3id.org/ontouml/2.0.0> ;
             rdfs:label "text"@en .


###  https://w3id.org/ontouml/2.0.0#upperBound
ontouml:upperBound rdf:type owl:DatatypeProperty ;
                   rdfs:domain ontouml:Cardinality ;
                   rdfs:range rdfs:Literal ;
                   rdfs:comment "An ontouml:Cardinality's upper bound must correspond to the one indicated by its ontouml:cardinalityValue property." ,
                                "E.g., if the ontouml:cardinalityValue set is [1..*] then the upper bound is '*'."@en ,
                                "Identifies the upper bound of an ontouml:Cardinality."@en ;
                   rdfs:isDefinedBy <https://w3id.org/ontouml/2.0.0> ;
                   rdfs:label "upper bound"@en .


###  https://w3id.org/ontouml/2.0.0#width
ontouml:width rdf:type owl:DatatypeProperty ;
              rdfs:domain ontouml:RectangularShape ;
              rdfs:range xsd:positiveInteger ;
              rdfs:comment "Indicates the width of an ontouml:RectangularShape that is represented in an ontouml:Diagram."@en ;
              rdfs:isDefinedBy <https://w3id.org/ontouml/2.0.0> ;
              rdfs:label "width"@en .


###  https://w3id.org/ontouml/2.0.0#xCoordinate
ontouml:xCoordinate rdf:type owl:DatatypeProperty ;
                    rdfs:domain ontouml:Point ;
                    rdfs:range xsd:integer ;
                    rdfs:comment "Is direct mapped to the metamodel's 'x' attribute of the Point class."@en ,
                                 "Relates an ontouml:Point to the value indicating the specific x (horizontal) coordinate of the top left position of an ontouml:RectangularShape."@en ;
                    rdfs:isDefinedBy <https://w3id.org/ontouml/2.0.0> ;
                    rdfs:label "x-coordinate"@en .


###  https://w3id.org/ontouml/2.0.0#yCoordinate
ontouml:yCoordinate rdf:type owl:DatatypeProperty ;
                    rdfs:domain ontouml:Point ;
                    rdfs:range xsd:integer ;
                    rdfs:comment "Is direct mapped to the metamodel's 'y' attribute of the Point class."@en ,
                                 "Relates an ontouml:Point to the value indicating the specific y (vertical) coordinate of the top left position of an ontouml:RectangularShape."@en ;
                    rdfs:isDefinedBy <https://w3id.org/ontouml/2.0.0> ;
                    rdfs:label "y-coordinate"@en .


#################################################################
#    Classes
#################################################################

###  http://purl.org/dc/terms/Standard
dct:Standard rdf:type owl:Class .


###  http://xmlns.com/foaf/0.1/Organization
foaf:Organization rdf:type owl:Class .


###  https://w3id.org/ontouml/2.0.0#AggregationKind
ontouml:AggregationKind rdf:type owl:Class ;
                        owl:equivalentClass [ rdf:type owl:Class ;
                                              owl:oneOf ( ontouml:composite
                                                          ontouml:none
                                                          ontouml:shared
                                                        )
                                            ] ;
                        rdfs:comment "Groups all possible aggregation kinds to which an ontouml:Property can be related."@en ,
                                     "This class is an enumeration of its individuals, which are: ontouml:composite, ontouml:none, and ontouml:shared."@en ;
                        rdfs:isDefinedBy <https://w3id.org/ontouml/2.0.0> ;
                        rdfs:label "Aggregation Kind"@en .


###  https://w3id.org/ontouml/2.0.0#BinaryConnectorView
ontouml:BinaryConnectorView rdf:type owl:Class ;
                            rdfs:subClassOf ontouml:View ;
                            owl:disjointUnionOf ( ontouml:BinaryRelationView
                                                  ontouml:GeneralizationView
                                                ) ;
                            rdfs:comment "An ontouml:View element that represents the single occurrence of a binary connector (e.g., a binary ontouml:Relation, or an ontouml:Generalization) in an ontouml:Diagram."@en ;
                            rdfs:isDefinedBy <https://w3id.org/ontouml/2.0.0> ;
                            rdfs:label "Binary Connector View"@en .


###  https://w3id.org/ontouml/2.0.0#BinaryRelation
ontouml:BinaryRelation rdf:type owl:Class ;
                       rdfs:subClassOf ontouml:Relation ;
                       rdfs:comment """An ontouml:Relation that defines the properties of a set of binary relations of the subject domain.

Examples include "studies in", and derivation relations (e.g., between material relations and relators).

A binary relation may either connect two classes, or a relation (as source) and a class (as class) in the case of ontouml:derivation relations connecting descriptive relations to the classes that serve as their truthmakers (as in the relation between the material relation "studies in" and the "Enrollment" relator)."""@en ;
                       rdfs:isDefinedBy <https://w3id.org/ontouml/2.0.0> ;
                       rdfs:label "Binary Relation"@en ;
                       rdfs:seeAlso ontouml:derivation, <https://doi.org/10.1007/978-3-030-33223-5_4> .


###  https://w3id.org/ontouml/2.0.0#BinaryRelationView
ontouml:BinaryRelationView rdf:type owl:Class ;
                           rdfs:subClassOf ontouml:BinaryConnectorView ;
                           rdfs:comment "An ontouml:View element that represents the single occurrence of a ontouml:BinaryRelation in an ontouml:Diagram."@en ;
                           rdfs:isDefinedBy <https://w3id.org/ontouml/2.0.0> ;
                           rdfs:label "Binary Relation View"@en .


###  https://w3id.org/ontouml/2.0.0#Cardinality
ontouml:Cardinality rdf:type owl:Class ;
                    rdfs:comment "Represents the cardinality of an ontouml:Property through its data property ontouml:cardinalityValue."@en ;
                    rdfs:isDefinedBy <https://w3id.org/ontouml/2.0.0> ;
                    rdfs:label "Cardinality"@en .


###  https://w3id.org/ontouml/2.0.0#Class
ontouml:Class rdf:type owl:Class ;
              rdfs:subClassOf ontouml:Classifier ,
                              [ owl:intersectionOf ( [ rdf:type owl:Restriction ;
                                                       owl:onProperty ontouml:stereotype ;
                                                       owl:allValuesFrom ontouml:ClassStereotype
                                                     ]
                                                     [ rdf:type owl:Restriction ;
                                                       owl:onProperty ontouml:stereotype ;
                                                       owl:qualifiedCardinality "1"^^xsd:nonNegativeInteger ;
                                                       owl:onClass ontouml:ClassStereotype
                                                     ]
                                                   ) ;
                                rdf:type owl:Class
                              ] ;
              rdfs:comment """An ontouml:Classifier that defines the properties of a set of \"individualized\" entities (i.e., non-relational) of the subject domain.
              
Examples include \"Person\", \"Enrollment\", and \"Grade\".

The instances of a class may include entities such as objects (e.g., people, organizations, vehicles), reified properties (e.g., leafs' colors, agents' intentions, enrollments), and bare values (e.g., a number or a literal)."""@en ;
              rdfs:isDefinedBy <https://w3id.org/ontouml/2.0.0> ;
              rdfs:label "Class"@en .


###  https://w3id.org/ontouml/2.0.0#ClassStereotype
ontouml:ClassStereotype rdf:type owl:Class ;
                        owl:equivalentClass [ rdf:type owl:Class ;
                                              owl:oneOf ( ontouml:abstract
                                                          ontouml:category
                                                          ontouml:collective
                                                          ontouml:datatype
                                                          ontouml:enumeration
                                                          ontouml:event
                                                          ontouml:historicalRole
                                                          ontouml:historicalRoleMixin
                                                          ontouml:kind
                                                          ontouml:mixin
                                                          ontouml:mode
                                                          ontouml:phase
                                                          ontouml:phaseMixin
                                                          ontouml:quality
                                                          ontouml:quantity
                                                          ontouml:relator
                                                          ontouml:role
                                                          ontouml:roleMixin
                                                          ontouml:situation
                                                          ontouml:subkind
                                                          ontouml:type
                                                        )
                                            ] ;
                        rdfs:subClassOf ontouml:Stereotype ;
                        rdfs:comment "Aggregates all possible instances that can be assigned via an ontouml:stereotype property to an ontouml:Class."@en ,
                                     "This class is an enumeration of its individuals, which are: ontouml:abstract, ontouml:category, ontouml:collective, ontouml:datatype, ontouml:enumeration, ontouml:event, ontouml:historicalRole, ontouml:historicalRoleMixin, ontouml:kind, ontouml:mixin, ontouml:mode, ontouml:phase, ontouml:phaseMixin, ontouml:quality, ontouml:quantity, ontouml:relator, ontouml:role, ontouml:roleMixin, ontouml:situation, ontouml:subkind, and ontouml:type."@en ;
                        rdfs:isDefinedBy <https://w3id.org/ontouml/2.0.0> ;
                        rdfs:label "Class Stereotype"@en .


###  https://w3id.org/ontouml/2.0.0#ClassView
ontouml:ClassView rdf:type owl:Class ;
                  rdfs:subClassOf ontouml:View ;
                  rdfs:comment "An ontouml:View element that represents the single occurrence of an ontouml:Class in an ontouml:Diagram."@en ;
                  rdfs:isDefinedBy <https://w3id.org/ontouml/2.0.0> ;
                  rdfs:label "Class View"@en .


###  https://w3id.org/ontouml/2.0.0#Classifier
ontouml:Classifier rdf:type owl:Class ;
                   rdfs:subClassOf ontouml:DecoratableElement ;
                   owl:disjointUnionOf ( ontouml:Class
                                         ontouml:Relation
                                       ) ;
                   rdfs:comment "An ontouml:DecoratableElement (either an ontouml:Class or an ontouml:Relation) that defines properties exhibited by its instances."@en ;
                   rdfs:isDefinedBy <https://w3id.org/ontouml/2.0.0> ;
                   rdfs:label "Classifier"@en ;
                   rdfs:seeAlso ontouml:Class ,
                                ontouml:Relation .


###  https://w3id.org/ontouml/2.0.0#DecoratableElement
ontouml:DecoratableElement rdf:type owl:Class ;
                           rdfs:subClassOf ontouml:ModelElement ;
                           owl:disjointUnionOf ( ontouml:Classifier
                                                 ontouml:Property
                                               ) ;
                           rdfs:comment """An ontouml:ModelElement that can be decorated with a stereotype to identify its ontological properties according to UFO.

Examples include a class decorated with the stereotype \"kind\" identifying it as a type of objects that provides an identity principle to its instances."""@en ;
                           rdfs:isDefinedBy <https://w3id.org/ontouml/2.0.0> ;
                           rdfs:label "Decoratable Element"@en .


###  https://w3id.org/ontouml/2.0.0#Diagram
ontouml:Diagram rdf:type owl:Class ;
                rdfs:subClassOf ontouml:NamedElement ;
                rdfs:comment "An ontouml:NamedElement that contains the visual representation of an OntoUML model or of a portion of it."@en ;
                rdfs:isDefinedBy <https://w3id.org/ontouml/2.0.0> ;
                rdfs:label "Diagram"@en .


###  https://w3id.org/ontouml/2.0.0#Diamond
ontouml:Diamond rdf:type owl:Class ;
                rdfs:subClassOf ontouml:RectangularShape .


###  https://w3id.org/ontouml/2.0.0#Generalization
ontouml:Generalization rdf:type owl:Class ;
                       rdfs:subClassOf ontouml:ModelElement ;
                       rdfs:comment """An ontouml:ModelElement that represents the generalization of a specific classifier into a general classifier. When read in the inverse direction, an ontouml:Generalization is referred to as a specialization.

Examples include the generalization of a specific class \"Student\" into a general class \"Person,\" and the generalization of a specific relation \"close friends with\" into a general relation \"friends with\".

A generalization can only connect two classifiers of the same type, i.e., it can either connect two ontouml:Class elements or two ontouml:Relation elements."""@en ;
                       rdfs:isDefinedBy <https://w3id.org/ontouml/2.0.0> ;
                       rdfs:label "Generalization"@en .


###  https://w3id.org/ontouml/2.0.0#GeneralizationSet
ontouml:GeneralizationSet rdf:type owl:Class ;
                          rdfs:subClassOf ontouml:ModelElement ;
                          rdfs:comment """An ontouml:ModelElement that represents a group of connected ontouml:Generalization elements. An ontouml:GeneralizationSet can define disjoint and/or complete constraints over the generalizations it groups.

Examples include the incomplete (i.e., non-complete) and overlapping (i.e., non-disjoint) generalization set of \"Person\" into \"Student\" and \"Teacher\", and the disjoint and complete generalization set of \"Person\" into \"Child\" and \"Adult\".

All ontouml:Generalization element in the ontouml:GeneralizationSet must share a common general ontouml:Classifier."""@en ;
                          rdfs:isDefinedBy <https://w3id.org/ontouml/2.0.0> ;
                          rdfs:label "Generalization Set"@en ;
                          rdfs:seeAlso ontouml:GeneralizationSet .


###  https://w3id.org/ontouml/2.0.0#GeneralizationSetView
ontouml:GeneralizationSetView rdf:type owl:Class ;
                              rdfs:subClassOf ontouml:View ;
                              rdfs:comment "An ontouml:View element that represents the single occurrence of an ontouml:Class in an ontouml:Diagram."@en ;
                              rdfs:isDefinedBy <https://w3id.org/ontouml/2.0.0> ;
                              rdfs:label "GeneralizationSetView"@en .


###  https://w3id.org/ontouml/2.0.0#GeneralizationView
ontouml:GeneralizationView rdf:type owl:Class ;
                           rdfs:subClassOf ontouml:BinaryConnectorView ;
                           rdfs:comment "Represents the diagramation (i.e., the visual representation) of an ontouml:Generalization in a given ontouml:Diagram."@en ;
                           rdfs:isDefinedBy <https://w3id.org/ontouml/2.0.0> ;
                           rdfs:label "Generalization View"@en .


###  https://w3id.org/ontouml/2.0.0#Link
ontouml:Link rdf:type owl:Class ;
             rdfs:subClassOf ontouml:ModelElement ;
             rdfs:comment "An ontouml:ModelElement that connects an ontouml:Note to the ontouml:ModelElement it concerns."@en ;
             rdfs:isDefinedBy <https://w3id.org/ontouml/2.0.0> ;
             rdfs:label "Link"@en .


###  https://w3id.org/ontouml/2.0.0#LinkView
ontouml:LinkView rdf:type owl:Class ;
                 rdfs:subClassOf ontouml:BinaryConnectorView ;
                 rdfs:comment "An ontouml:View element that represents the single occurrence of an ontouml:Link in an ontouml:Diagram."@en ;
                 rdfs:isDefinedBy <https://w3id.org/ontouml/2.0.0> ;
                 rdfs:label "Link View"@en .


###  https://w3id.org/ontouml/2.0.0#Literal
ontouml:Literal rdf:type owl:Class ;
                rdfs:subClassOf ontouml:ModelElement ;
                rdfs:comment "An ontouml:ModelElement that represents a specific value within an enumerated set of values within an ontouml:Class with the ontouml:stereotype ontouml:enumeration. Examples include each letter in an A to F letter grading scale, listed in a class \"Letter Grade\" decorated with the stereotype \"enumeration\"."@en ;
                rdfs:isDefinedBy <https://w3id.org/ontouml/2.0.0> ;
                rdfs:label "Literal"@en ;
                rdfs:seeAlso ontouml:Class ,
                             ontouml:enumeration .


###  https://w3id.org/ontouml/2.0.0#ModelElement
ontouml:ModelElement rdf:type owl:Class ;
                     rdfs:subClassOf ontouml:NamedElement ;
                     owl:disjointUnionOf ( ontouml:DecoratableElement
                                           ontouml:Generalization
                                           ontouml:GeneralizationSet
                                           ontouml:Literal
                                           ontouml:Note
                                           ontouml:Package
                                         ) ;
                     rdfs:comment "An ontouml:NamedElement that represents an element of the language's abstract syntax (e.g., an ontouml:Class, an ontouml:Relation, or an ontouml:Generalization)."@en ;
                     rdfs:isDefinedBy <https://w3id.org/ontouml/2.0.0> ;
                     rdfs:label "Model Element"@en .


###  https://w3id.org/ontouml/2.0.0#NamedElement
ontouml:NamedElement rdf:type owl:Class ;
                     rdfs:subClassOf ontouml:OntoumlElement ;
                     owl:disjointUnionOf ( ontouml:ModelElement
                                           ontouml:Project
                                         ) ;
                     rdfs:comment "An ontouml:ontoumlElement that can be attributed a name and other descriptive information."@en ;
                     rdfs:isDefinedBy <https://w3id.org/ontouml/2.0.0> ;
                     rdfs:label "Named Element"@en .


###  https://w3id.org/ontouml/2.0.0#NaryRelation
ontouml:NaryRelation rdf:type owl:Class ;
                     rdfs:subClassOf ontouml:Relation ;
                     rdfs:comment """An ontouml:Relation that defines the properties of a set of relations of the subject domain that connect more than two members.

Examples include "studies in", "buys product from" (ternary relation), and derivation relations (e.g., between material relations and relators)."""@en ;
                     rdfs:isDefinedBy <https://w3id.org/ontouml/2.0.0> ;
                     rdfs:label "N-ary Relation"@en .


###  https://w3id.org/ontouml/2.0.0#NaryRelationView
ontouml:NaryRelationView rdf:type owl:Class ;
                         rdfs:subClassOf ontouml:View ;
                         rdfs:comment "An ontouml:View element that represents the single occurrence of an ontouml:NaryRelation in an ontouml:Diagram."@en ;
                         rdfs:isDefinedBy <https://w3id.org/ontouml/2.0.0> ;
                         rdfs:label "N-ary Relation View"@en .


###  https://w3id.org/ontouml/2.0.0#Note
ontouml:Note rdf:type owl:Class ;
             rdfs:subClassOf ontouml:ModelElement ;
             rdfs:comment "An ontouml:ModelElement that contains an annotation about the ontology or some of its elements. A note can also be used to represent a constraint in both natural or structured language (i.e., first-order logic, or OCL)."@en ;
             rdfs:isDefinedBy <https://w3id.org/ontouml/2.0.0> ;
             rdfs:label "Note"@en .


###  https://w3id.org/ontouml/2.0.0#NoteView
ontouml:NoteView rdf:type owl:Class ;
                 rdfs:subClassOf ontouml:View ;
                 rdfs:comment "An ontouml:View element that represents the single occurrence of an ontouml:Note in an ontouml:Diagram."@en ;
                 rdfs:isDefinedBy <https://w3id.org/ontouml/2.0.0> ;
                 rdfs:label "Note View"@en .


###  https://w3id.org/ontouml/2.0.0#OntologicalNature
ontouml:OntologicalNature rdf:type owl:Class ;
                          owl:equivalentClass [ rdf:type owl:Class ;
                                                owl:oneOf ( ontouml:abstractNature
                                                            ontouml:collectiveNature
                                                            ontouml:eventNature
                                                            ontouml:extrinsicModeNature
                                                            ontouml:functionalComplexNature
                                                            ontouml:intrinsicModeNature
                                                            ontouml:qualityNature
                                                            ontouml:quantityNature
                                                            ontouml:relatorNature
                                                            ontouml:situationNature
                                                            ontouml:typeNature
                                                          )
                                              ] ;
                          rdfs:comment "Collection of individuals that represent fundamental conceptual modeling issues according to the Unified Foundational Ontology (UFO) theory."@en ,
                                       "This class is an enumeration of its individuals, which are: ontouml:abstractNature, ontouml:collectiveNature, ontouml:eventNature, ontouml:extrinsicModeNature, ontouml:functionalComplexNature, ontouml:intrinsicModeNature, ontouml:qualityNature, ontouml:quantityNature, ontouml:relatorNature, ontouml:situationNature, and ontouml:typeNature."@en ;
                          rdfs:isDefinedBy <https://w3id.org/ontouml/2.0.0> ;
                          rdfs:label "Ontological Nature"@en ;
                          rdfs:seeAlso <https://doi.org/10.3233/AO-150157> .


###  https://w3id.org/ontouml/2.0.0#OntoumlElement
ontouml:OntoumlElement rdf:type owl:Class ;
                       rdfs:comment "An identified element of an OntoUML ontology according to the OntoUML Metamodel, which includes projects, model elements, diagrams, views, and shapes."@en ;
                       rdfs:isDefinedBy <https://w3id.org/ontouml/2.0.0> ;
                       rdfs:label "OntoUML Element"@en .


###  https://w3id.org/ontouml/2.0.0#Package
ontouml:Package rdf:type owl:Class ;
                rdfs:subClassOf ontouml:ModelElement ;
                rdfs:comment """An ontouml:ModelElement that groups other model elements referred to as \"packageable elements.\" Package elements are used to perform the modularization of an ontology.
                
While the OntoUML Metamodel does not require package elements to follow a tree structure (i.e., it allows overlapping packages), ontologies that require UML representations should adhere to this constraint for compatibility."""@en ;
                rdfs:isDefinedBy <https://w3id.org/ontouml/2.0.0> ;
                rdfs:label "Package"@en .


###  https://w3id.org/ontouml/2.0.0#PackageView
ontouml:PackageView rdf:type owl:Class ;
                    rdfs:subClassOf ontouml:View ;
                    rdfs:comment "An ontouml:View element that represents the single occurrence of an ontouml:Package in an ontouml:Diagram."@en ;
                    rdfs:isDefinedBy <https://w3id.org/ontouml/2.0.0> ;
                    rdfs:label "Package View"@en .


###  https://w3id.org/ontouml/2.0.0#Path
ontouml:Path rdf:type owl:Class ;
             rdfs:subClassOf ontouml:Shape ;
             rdfs:comment "A list of connected ontouml:Point values to represent an ontouml:ElementView's shape."@en ;
             rdfs:isDefinedBy <https://w3id.org/ontouml/2.0.0> ;
             rdfs:label "Path"@en .


###  https://w3id.org/ontouml/2.0.0#Point
ontouml:Point rdf:type owl:Class ;
              rdfs:comment "Contains the ontouml:xCoordinate value and ontouml:yCoordinate value. These values represent the top left position of an ontouml:RectangularShape, to which the ontouml:Point is related vian ontouml:topLeftPosition property."@en ;
              rdfs:isDefinedBy <https://w3id.org/ontouml/2.0.0> ;
              rdfs:label "Point"@en .


###  https://w3id.org/ontouml/2.0.0#Project
ontouml:Project rdf:type owl:Class ;
                rdfs:subClassOf ontouml:NamedElement ;
                rdfs:comment "An ontouml:NamedElement that serves as the container of an entire OntoUML ontology, including the elements of both the abstract syntax (i.e., model elements) and the concrete syntax (i.e., diagrams, view, and shapes)."@en ;
                rdfs:isDefinedBy <https://w3id.org/ontouml/2.0.0> ;
                rdfs:label "Project"@en .


###  https://w3id.org/ontouml/2.0.0#Property
ontouml:Property rdf:type owl:Class ;
                 rdfs:subClassOf ontouml:DecoratableElement ,
                                 [ owl:intersectionOf ( [ rdf:type owl:Restriction ;
                                                          owl:onProperty ontouml:stereotype ;
                                                          owl:allValuesFrom ontouml:PropertyStereotype
                                                        ]
                                                        [ rdf:type owl:Restriction ;
                                                          owl:onProperty ontouml:stereotype ;
                                                          owl:maxQualifiedCardinality "1"^^xsd:nonNegativeInteger ;
                                                          owl:onClass ontouml:PropertyStereotype
                                                        ]
                                                      ) ;
                                   rdf:type owl:Class
                                 ] ;
                 rdfs:comment """An ontouml:DecoratableElement that represents an attribute of an ontouml:Class, or one end of an ontouml:Relation.

Examples include the attribute \"name\" of the class \"Person\", and the ends of the binary relation \"studies in\" connected to the classes \"Student\" and \"University.\"

Instances of class and relation elements bear values for the properties these classifiers contain, according to the constraints specified within each property. For example, the value assigned to a property in an instance must be itself an instance of the classifier in property type."""@en ;
                 rdfs:isDefinedBy <https://w3id.org/ontouml/2.0.0> ;
                 rdfs:label "Property"@en .


###  https://w3id.org/ontouml/2.0.0#PropertyStereotype
ontouml:PropertyStereotype rdf:type owl:Class ;
                           owl:equivalentClass [ rdf:type owl:Class ;
                                                 owl:oneOf ( ontouml:begin
                                                             ontouml:end
                                                           )
                                               ] ;
                           rdfs:subClassOf ontouml:Stereotype ;
                           rdfs:comment "Aggregates all possible instances that can be assigned via an ontouml:stereotype property to an ontouml:Property."@en ,
                                        "This class is an enumeration of its individuals, which are: ontouml:begin, and ontouml:end."@en ;
                           rdfs:isDefinedBy <https://w3id.org/ontouml/2.0.0> ;
                           rdfs:label "Property Stereotype"@en .


###  https://w3id.org/ontouml/2.0.0#Rectangle
ontouml:Rectangle rdf:type owl:Class ;
                  rdfs:subClassOf ontouml:RectangularShape ;
                  rdfs:comment "A particular type of ontouml:RectangularShape, mainly used to represent entities of type ontouml:Class."@en ;
                  rdfs:isDefinedBy <https://w3id.org/ontouml/2.0.0> ;
                  rdfs:label "Rectangle"@en .


###  https://w3id.org/ontouml/2.0.0#RectangularShape
ontouml:RectangularShape rdf:type owl:Class ;
                         rdfs:subClassOf ontouml:Shape ;
                         owl:disjointUnionOf ( ontouml:Rectangle
                                               ontouml:Text
                                             ) ;
                         rdfs:comment "Represents a rectangular shape in a given ontouml:Diagram."@en ;
                         rdfs:isDefinedBy <https://w3id.org/ontouml/2.0.0> ;
                         rdfs:label "Rectangular Shape"@en .


###  https://w3id.org/ontouml/2.0.0#Relation
ontouml:Relation rdf:type owl:Class ;
                 rdfs:subClassOf ontouml:Classifier ,
                                 [ owl:intersectionOf ( [ rdf:type owl:Restriction ;
                                                          owl:onProperty ontouml:stereotype ;
                                                          owl:allValuesFrom ontouml:RelationStereotype
                                                        ]
                                                        [ rdf:type owl:Restriction ;
                                                          owl:onProperty ontouml:stereotype ;
                                                          owl:maxQualifiedCardinality "1"^^xsd:nonNegativeInteger ;
                                                          owl:onClass ontouml:RelationStereotype
                                                        ]
                                                      ) ;
                                   rdf:type owl:Class
                                 ] ;
                 rdfs:comment """An ontouml:Classifier that defines the properties of a set of relations of the subject domain.

Examples include "studies in", "buys product from" (ternary relation), and derivation relations (e.g., between material relations and relators)."""@en ;
                 rdfs:isDefinedBy <https://w3id.org/ontouml/2.0.0> ;
                 rdfs:label "Relation"@en .


###  https://w3id.org/ontouml/2.0.0#RelationStereotype
ontouml:RelationStereotype rdf:type owl:Class ;
                           owl:equivalentClass [ rdf:type owl:Class ;
                                                 owl:oneOf ( ontouml:bringsAbout
                                                             ontouml:characterization
                                                             ontouml:comparative
                                                             ontouml:componentOf
                                                             ontouml:creation
                                                             ontouml:derivation
                                                             ontouml:externalDependence
                                                             ontouml:historicalDependence
                                                             ontouml:instantiation
                                                             ontouml:manifestation
                                                             ontouml:material
                                                             ontouml:mediation
                                                             ontouml:memberOf
                                                             ontouml:participation
                                                             ontouml:participational
                                                             ontouml:subCollectionOf
                                                             ontouml:subQuantityOf
                                                             ontouml:termination
                                                             ontouml:triggers
                                                           )
                                               ] ;
                           rdfs:subClassOf ontouml:Stereotype ;
                           rdfs:comment "Aggregates all possible instances that can be assigned via an ontouml:stereotype property to an ontouml:Relation."@en ,
                                        "This class is an enumeration of its individuals, which are: ontouml:bringsAbout, ontouml:characterization, ontouml:comparative, ontouml:componentOf, ontouml:creation, ontouml:derivation, ontouml:externalDependence, ontouml:historicalDependence, ontouml:instantiation, ontouml:manifestation, ontouml:material, ontouml:mediation, ontouml:memberOf, ontouml:participation, ontouml:participational, ontouml:subCollectionOf, ontouml:subQuantityOf, ontouml:termination, and ontouml:triggers."@en ;
                           rdfs:isDefinedBy <https://w3id.org/ontouml/2.0.0> ;
                           rdfs:label "Relation Stereotype"@en .


###  https://w3id.org/ontouml/2.0.0#Shape
ontouml:Shape rdf:type owl:Class ;
              rdfs:subClassOf ontouml:OntoumlElement ;
              owl:disjointUnionOf ( ontouml:Path
                                    ontouml:RectangularShape
                                  ) ;
              rdfs:comment "An ontouml:OntoumlElement that identifies how to render an ontouml:View (or a portion of one) in an ontouml:Diagram."@en ;
              rdfs:isDefinedBy <https://w3id.org/ontouml/2.0.0> ;
              rdfs:label "Shape"@en .


###  https://w3id.org/ontouml/2.0.0#Stereotype
ontouml:Stereotype rdf:type owl:Class ;
                   owl:disjointUnionOf ( ontouml:ClassStereotype
                                         ontouml:PropertyStereotype
                                         ontouml:RelationStereotype
                                       ) ;
                   rdfs:comment "Indicates meta-properties of classes, properties, or relations."@en ;
                   rdfs:isDefinedBy <https://w3id.org/ontouml/2.0.0> ;
                   rdfs:label "Stereotype"@en .


###  https://w3id.org/ontouml/2.0.0#Text
ontouml:Text rdf:type owl:Class ;
             rdfs:subClassOf ontouml:RectangularShape ;
             rdfs:comment "An ontouml:RectangularShape used to represent some textual information in an ontouml:Diagram."@en ;
             rdfs:isDefinedBy <https://w3id.org/ontouml/2.0.0> ;
             rdfs:label "Text"@en .


###  https://w3id.org/ontouml/2.0.0#View
ontouml:View rdf:type owl:Class ;
             rdfs:subClassOf ontouml:OntoumlElement ;
             rdfs:comment """An ontouml:OntoumlElement that represents a single ontouml:ModelElement in a ontouml:Diagram.

A view element connects a model element to the shapes in a diagram necessary to represent a single occurrence of it. For example, an n-ary relation view connects a single relation element to one diamond and a set of paths that represent a single occurrence of it in a diagram. Multiple views can represent multiple occurrences of an element in the same diagram.
      
A view element is responsible for what portions of a model element are present in a single diagram representation (e.g., whether the cardinality of a property is shown), unlike a shape, which is responsible aspects of the actual drawing (e.g., how to render a portion of a view, in which position, and with which dimensions)."""@en ;
             rdfs:isDefinedBy <https://w3id.org/ontouml/2.0.0> ;
             rdfs:label "Element View"@en ;
             rdfs:seeAlso ontouml:Shape .


#################################################################
#    Individuals
#################################################################

###  https://w3id.org/ontouml
<https://w3id.org/ontouml> rdf:type owl:NamedIndividual ,
                                    dct:Standard .


###  https://w3id.org/ontouml/2.0.0#abstract
ontouml:abstract rdf:type owl:NamedIndividual ,
                          ontouml:ClassStereotype ;
                 rdfs:comment "An individual of the ontouml:ClassStereotype used to assign the corresponding stereotype to a given ontouml:Class."@en ;
                 rdfs:isDefinedBy <https://w3id.org/ontouml/2.0.0> ;
                 rdfs:label "abstract"@en .


###  https://w3id.org/ontouml/2.0.0#abstractNature
ontouml:abstractNature rdf:type owl:NamedIndividual ,
                                ontouml:OntologicalNature ;
                       rdfs:comment "Indicates that the restricted type includes abstract individuals among its instances."@en ;
                       rdfs:isDefinedBy <https://w3id.org/ontouml/2.0.0> ;
                       rdfs:label "abstract nature"@en .


###  https://w3id.org/ontouml/2.0.0#begin
ontouml:begin rdf:type owl:NamedIndividual ,
                       ontouml:PropertyStereotype ;
              rdfs:comment "An individual of the ontouml:PropertyStereotype used to assign the corresponding stereotype to a given ontouml:Property."@en ;
              rdfs:isDefinedBy <https://w3id.org/ontouml/2.0.0> ;
              rdfs:label "begin"@en ;
              rdfs:seeAlso <https://doi.org/10.1007/978-3-030-33223-5_39> .


###  https://w3id.org/ontouml/2.0.0#bringsAbout
ontouml:bringsAbout rdf:type owl:NamedIndividual ,
                             ontouml:RelationStereotype ;
                    rdfs:comment "An individual of the ontouml:RelationStereotype used to assign the corresponding stereotype to a given ontouml:Relation."@en ;
                    rdfs:isDefinedBy <https://w3id.org/ontouml/2.0.0> ;
                    rdfs:label "brings about"@en ;
                    rdfs:seeAlso <https://doi.org/10.1007/978-3-030-33223-5_39> .


###  https://w3id.org/ontouml/2.0.0#category
ontouml:category rdf:type owl:NamedIndividual ,
                          ontouml:ClassStereotype ;
                 rdfs:comment "A rigid mixin that does not require a dependency to be specified. It is used to aggregate essential properties of individuals following different identity principles."@en ;
                 rdfs:isDefinedBy <https://w3id.org/ontouml/2.0.0> ;
                 rdfs:label "category"@en ;
                 rdfs:seeAlso "https://ontouml.readthedocs.io/en/latest/classes/nonsortals/category/index.html"^^xsd:anyURI .


###  https://w3id.org/ontouml/2.0.0#characterization
ontouml:characterization rdf:type owl:NamedIndividual ,
                                  ontouml:RelationStereotype ;
                         rdfs:comment "An ontouml:RelationStereotype attributed to a relation between a bearer type and its feature."@en ;
                         rdfs:isDefinedBy <https://w3id.org/ontouml/2.0.0> ;
                         rdfs:label "characterization"@en ;
                         rdfs:seeAlso <https://doi.org/10.1007/978-3-030-33223-5_4> ,
                                      "https://ontouml.readthedocs.io/en/latest/relationships/characterization/index.html"^^xsd:anyURI .


###  https://w3id.org/ontouml/2.0.0#collective
ontouml:collective rdf:type owl:NamedIndividual ,
                            ontouml:ClassStereotype ;
                   rdfs:comment "An ontouml:ClassStereotype used to represent rigid concepts that provide an identity principle for their instances."@en ;
                   rdfs:isDefinedBy <https://w3id.org/ontouml/2.0.0> ;
                   rdfs:label "collective"@en ;
                   rdfs:seeAlso "https://ontouml.readthedocs.io/en/latest/classes/sortals/collective/index.html"^^xsd:anyURI .


###  https://w3id.org/ontouml/2.0.0#collectiveNature
ontouml:collectiveNature rdf:type owl:NamedIndividual ,
                                  ontouml:OntologicalNature ;
                         rdfs:comment "Indicates that the restricted type includes collective individuals among its instances."@en ;
                         rdfs:isDefinedBy <https://w3id.org/ontouml/2.0.0> ;
                         rdfs:label "collective nature"@en .


###  https://w3id.org/ontouml/2.0.0#comparative
ontouml:comparative rdf:type owl:NamedIndividual ,
                             ontouml:RelationStereotype ;
                    rdfs:comment "The stereotype for comparative relations (e.g., heavier-than). Decorates relations that always hold between any two individuals bearing the same relevant quality."@en ;
                    rdfs:isDefinedBy <https://w3id.org/ontouml/2.0.0> ;
                    rdfs:label "comparative"@en ;
                    rdfs:seeAlso <https://doi.org/10.1007/978-3-030-33223-5_4> .


###  https://w3id.org/ontouml/2.0.0#componentOf
ontouml:componentOf rdf:type owl:NamedIndividual ,
                             ontouml:RelationStereotype ;
                    rdfs:comment "A parthood relation between two complexes."@en ;
                    rdfs:isDefinedBy <https://w3id.org/ontouml/2.0.0> ;
                    rdfs:label "component of"@en ;
                    rdfs:seeAlso "https://ontouml.readthedocs.io/en/latest/relationships/aggregations/componentOf/index.html"^^xsd:anyURI .


###  https://w3id.org/ontouml/2.0.0#composite
ontouml:composite rdf:type owl:NamedIndividual ,
                           ontouml:AggregationKind ;
                  rdfs:comment "The value denoting that an ontouml:Property represents a composite aggregation, i.e., a strong form of aggregation."@en ;
                  rdfs:isDefinedBy <https://w3id.org/ontouml/2.0.0> ;
                  rdfs:label "composite"@en .


###  https://w3id.org/ontouml/2.0.0#creation
ontouml:creation rdf:type owl:NamedIndividual ,
                          ontouml:RelationStereotype ;
                 rdfs:comment "An individual of the ontouml:RelationStereotype used to assign the corresponding stereotype to a given ontouml:Relation."@en ;
                 rdfs:isDefinedBy <https://w3id.org/ontouml/2.0.0> ;
                 rdfs:label "creation"@en ;
                 rdfs:seeAlso <https://doi.org/10.1007/978-3-030-33223-5_39> .


###  https://w3id.org/ontouml/2.0.0#datatype
ontouml:datatype rdf:type owl:NamedIndividual ,
                          ontouml:ClassStereotype ;
                 rdfs:comment "An individual of the ontouml:ClassStereotype used to assign the corresponding stereotype to a given ontouml:Class."@en ;
                 rdfs:isDefinedBy <https://w3id.org/ontouml/2.0.0> ;
                 rdfs:label "datatype"@en .


###  https://w3id.org/ontouml/2.0.0#derivation
ontouml:derivation rdf:type owl:NamedIndividual ,
                            ontouml:RelationStereotype ;
                   rdfs:comment "An individual of the ontouml:RelationStereotype used to assign the corresponding stereotype to a given ontouml:Relation."@en ;
                   rdfs:isDefinedBy <https://w3id.org/ontouml/2.0.0> ;
                   rdfs:label "derivation"@en .


###  https://w3id.org/ontouml/2.0.0#end
ontouml:end rdf:type owl:NamedIndividual ,
                     ontouml:PropertyStereotype ;
            rdfs:comment "An individual of the ontouml:PropertyStereotype used to assign the corresponding stereotype to a given ontouml:Property."@en ;
            rdfs:isDefinedBy <https://w3id.org/ontouml/2.0.0> ;
            rdfs:label "end"@en ;
            rdfs:seeAlso <https://doi.org/10.1007/978-3-030-33223-5_39> .


###  https://w3id.org/ontouml/2.0.0#enumeration
ontouml:enumeration rdf:type owl:NamedIndividual ,
                             ontouml:ClassStereotype ;
                    rdfs:comment "Represents the enumeration stereotype, having values represented using ontouml:Literal instances."@en ;
                    rdfs:isDefinedBy <https://w3id.org/ontouml/2.0.0> ;
                    rdfs:label "enumeration"@en .


###  https://w3id.org/ontouml/2.0.0#event
ontouml:event rdf:type owl:NamedIndividual ,
                       ontouml:ClassStereotype ;
              rdfs:comment "An individual of the ontouml:ClassStereotype used to assign the corresponding stereotype to a given ontouml:Class."@en ,
                           "Things that happen to or are performed by endurants (Casati and Varzi, 2015)."@en ;
              rdfs:isDefinedBy <https://w3id.org/ontouml/2.0.0> ;
              rdfs:label "event"@en ;
              rdfs:seeAlso <https://doi.org/10.1007/978-3-030-33223-5_39> .


###  https://w3id.org/ontouml/2.0.0#eventNature
ontouml:eventNature rdf:type owl:NamedIndividual ,
                             ontouml:OntologicalNature ;
                    rdfs:comment "Indicates that the restricted type includes event individuals among its instances."@en ;
                    rdfs:isDefinedBy <https://w3id.org/ontouml/2.0.0> ;
                    rdfs:label "event nature"@en .


###  https://w3id.org/ontouml/2.0.0#externalDependence
ontouml:externalDependence rdf:type owl:NamedIndividual ,
                                    ontouml:RelationStereotype ;
                           rdfs:comment "Identifies an endurant on which the extrinsicMode depends."@en ;
                           rdfs:isDefinedBy <https://w3id.org/ontouml/2.0.0> ;
                           rdfs:label "external dependence"@en ;
                           rdfs:seeAlso <https://doi.org/10.1007/978-3-030-33223-5_4> ,
                                        "https://nemo-ufes.github.io/gufo/#externallyDependsOn"^^xsd:anyURI .


###  https://w3id.org/ontouml/2.0.0#extrinsicModeNature
ontouml:extrinsicModeNature rdf:type owl:NamedIndividual ,
                                     ontouml:OntologicalNature ;
                            rdfs:comment "Identifies what inheres in a concrete individual and depends on others for its existence."@en ;
                            rdfs:isDefinedBy <https://w3id.org/ontouml/2.0.0> ;
                            rdfs:label "extrinsic mode nature"@en .


###  https://w3id.org/ontouml/2.0.0#functionalComplexNature
ontouml:functionalComplexNature rdf:type owl:NamedIndividual ,
                                         ontouml:OntologicalNature ;
                                rdfs:comment "Identifies the nature of a complex object whose parts (components) play different roles in its composition."@en ;
                                rdfs:isDefinedBy <https://w3id.org/ontouml/2.0.0> ;
                                rdfs:label "functional-complex nature"@en .


###  https://w3id.org/ontouml/2.0.0#historicalDependence
ontouml:historicalDependence rdf:type owl:NamedIndividual ,
                                      ontouml:RelationStereotype ;
                             rdfs:comment "Identifies a concrete individual on which another concrete individual depends historically."@en ;
                             rdfs:isDefinedBy <https://w3id.org/ontouml/2.0.0> ;
                             rdfs:label "historical dependence"@en ;
                             rdfs:seeAlso <https://doi.org/10.1007/978-3-030-33223-5_39> .


###  https://w3id.org/ontouml/2.0.0#historicalRole
ontouml:historicalRole rdf:type owl:NamedIndividual ,
                                ontouml:ClassStereotype ;
                       rdfs:comment "Denotes the role of an endurant in virtue of having participated in an event of a particular type."@en ;
                       rdfs:isDefinedBy <https://w3id.org/ontouml/2.0.0> ;
                       rdfs:label "historical role"@en ;
                       rdfs:seeAlso <https://doi.org/10.1007/978-3-030-33223-5_39> .


###  https://w3id.org/ontouml/2.0.0#historicalRoleMixin
ontouml:historicalRoleMixin rdf:type owl:NamedIndividual ,
                                     ontouml:ClassStereotype ;
                            rdfs:comment "Denotes the equivalent of historicalRole for types that aggregate instances with different identity principles."@en ;
                            rdfs:isDefinedBy <https://w3id.org/ontouml/2.0.0> ;
                            rdfs:label "historical role mixin"@en ;
                            rdfs:seeAlso <https://doi.org/10.1007/978-3-030-33223-5_39> .


###  https://w3id.org/ontouml/2.0.0#instantiation
ontouml:instantiation rdf:type owl:NamedIndividual ,
                               ontouml:RelationStereotype ;
                      rdfs:comment "An individual of the ontouml:RelationStereotype used to assign the corresponding stereotype to a given ontouml:Relation."@en ;
                      rdfs:isDefinedBy <https://w3id.org/ontouml/2.0.0> ;
                      rdfs:label "instantiation"@en .


###  https://w3id.org/ontouml/2.0.0#intrinsicModeNature
ontouml:intrinsicModeNature rdf:type owl:NamedIndividual ,
                                     ontouml:OntologicalNature ;
                            rdfs:comment "Indicates that the restricted type includes intrinsic mode individuals among its instances."@en ;
                            rdfs:isDefinedBy <https://w3id.org/ontouml/2.0.0> ;
                            rdfs:label "intrinsic mode nature"@en .


###  https://w3id.org/ontouml/2.0.0#kind
ontouml:kind rdf:type owl:NamedIndividual ,
                      ontouml:ClassStereotype ;
             rdfs:comment "Used to represent rigid concepts that provide an identity principle for their instances and do not require a relational dependency."@en ;
             rdfs:isDefinedBy <https://w3id.org/ontouml/2.0.0> ;
             rdfs:label "kind"@en ;
             rdfs:seeAlso "https://ontouml.readthedocs.io/en/latest/classes/sortals/kind/index.html"^^xsd:anyURI .


###  https://w3id.org/ontouml/2.0.0#manifestation
ontouml:manifestation rdf:type owl:NamedIndividual ,
                               ontouml:RelationStereotype ;
                      rdfs:comment "An individual of the ontouml:RelationStereotype used to assign the corresponding stereotype to a given ontouml:Relation."@en ;
                      rdfs:isDefinedBy <https://w3id.org/ontouml/2.0.0> ;
                      rdfs:label "manifestation"@en .


###  https://w3id.org/ontouml/2.0.0#material
ontouml:material rdf:type owl:NamedIndividual ,
                          ontouml:RelationStereotype ;
                 rdfs:comment "Identifies relations that have material structure on their own and include examples such as employments, kisses, enrollments, flight, connections and commitments."@en ;
                 rdfs:isDefinedBy <https://w3id.org/ontouml/2.0.0> ;
                 rdfs:label "material"@en ;
                 rdfs:seeAlso <https://doi.org/10.1007/978-3-030-33223-5_4> ,
                              "https://ontouml.readthedocs.io/en/latest/relationships/material/index.html"^^xsd:anyURI .


###  https://w3id.org/ontouml/2.0.0#mediation
ontouml:mediation rdf:type owl:NamedIndividual ,
                           ontouml:RelationStereotype ;
                  rdfs:comment "A type of existential dependence relation (a form of nonfunctional inherence). It can be derived from the relation between the relata and the qua individuals that compose the relator and that inhere in the relata."@en ;
                  rdfs:isDefinedBy <https://w3id.org/ontouml/2.0.0> ;
                  rdfs:label "mediation"@en ;
                  rdfs:seeAlso <https://doi.org/10.1007/978-3-030-33223-5_4> ,
                               "https://ontouml.readthedocs.io/en/latest/relationships/mediation/index.html"^^xsd:anyURI .


###  https://w3id.org/ontouml/2.0.0#memberOf
ontouml:memberOf rdf:type owl:NamedIndividual ,
                          ontouml:RelationStereotype ;
                 rdfs:comment "A parthood relation between a functional complex or a Collective (as a part) and a Collective (as a whole)."@en ;
                 rdfs:isDefinedBy <https://w3id.org/ontouml/2.0.0> ;
                 rdfs:label "member of"@en ;
                 rdfs:seeAlso "https://ontouml.readthedocs.io/en/latest/relationships/aggregations/memberOf/index.html"^^xsd:anyURI .


###  https://w3id.org/ontouml/2.0.0#mixin
ontouml:mixin rdf:type owl:NamedIndividual ,
                       ontouml:ClassStereotype ;
              rdfs:comment "Represents a semi-rigid type, i.e., it behaves as a rigid type for some individuals and as an anti-rigid one for others."@en ;
              rdfs:isDefinedBy <https://w3id.org/ontouml/2.0.0> ;
              rdfs:label "mixin"@en ;
              rdfs:seeAlso "https://ontouml.readthedocs.io/en/latest/classes/nonsortals/mixin/index.html"^^xsd:anyURI .


###  https://w3id.org/ontouml/2.0.0#mode
ontouml:mode rdf:type owl:NamedIndividual ,
                      ontouml:ClassStereotype ;
             rdfs:comment "A particular type of intrinsic property that has no structured value."@en ;
             rdfs:isDefinedBy <https://w3id.org/ontouml/2.0.0> ;
             rdfs:label "mode"@en ;
             rdfs:seeAlso "https://ontouml.readthedocs.io/en/latest/classes/aspects/mode/index.html"^^xsd:anyURI .


###  https://w3id.org/ontouml/2.0.0#none
ontouml:none rdf:type owl:NamedIndividual ,
                      ontouml:AggregationKind ;
             rdfs:comment "Denotes that an ontouml:Property is neither ontouml:shared nor ontouml:composite, but just an aggregation."@en ;
             rdfs:isDefinedBy <https://w3id.org/ontouml/2.0.0> ;
             rdfs:label "none"@en .


###  https://w3id.org/ontouml/2.0.0#participation
ontouml:participation rdf:type owl:NamedIndividual ,
                               ontouml:RelationStereotype ;
                      rdfs:comment "A relation for representing when an event depends on a single object."@en ;
                      rdfs:isDefinedBy <https://w3id.org/ontouml/2.0.0> ;
                      rdfs:label "participation"@en ;
                      rdfs:seeAlso <https://doi.org/10.1007/978-3-030-33223-5_39> .


###  https://w3id.org/ontouml/2.0.0#participational
ontouml:participational rdf:type owl:NamedIndividual ,
                                 ontouml:RelationStereotype ;
                        rdfs:comment "Denotes a kind of event decomposition."@en ;
                        rdfs:isDefinedBy <https://w3id.org/ontouml/2.0.0> ;
                        rdfs:label "participational"@en ;
                        rdfs:seeAlso <https://doi.org/10.1007/978-3-030-33223-5_39> .


###  https://w3id.org/ontouml/2.0.0#phase
ontouml:phase rdf:type owl:NamedIndividual ,
                       ontouml:ClassStereotype ;
              rdfs:comment "Used to represent anti-rigid subtypes of identity providers (Kind, Collective, Quantity, Relator, Mode, and Quantity) that are instantiated by changes in intrinsic properties (e.g., the age of a person, the color of an object, the condition of a car).Phases always come in partitions."@en ;
              rdfs:isDefinedBy <https://w3id.org/ontouml/2.0.0> ;
              rdfs:label "phase"@en ;
              rdfs:seeAlso "https://ontouml.readthedocs.io/en/latest/classes/sortals/phase/index.html"^^xsd:anyURI .


###  https://w3id.org/ontouml/2.0.0#phaseMixin
ontouml:phaseMixin rdf:type owl:NamedIndividual ,
                            ontouml:ClassStereotype ;
                   rdfs:comment "The equivalent of Phase for types that aggregate instances with different identity principles. A class stereotyped as PhaseMixin is also an anti-rigid type. PhaseMixin is similar semantically to RoleMixin with the difference in relational dependency."@en ;
                   rdfs:isDefinedBy <https://w3id.org/ontouml/2.0.0> ;
                   rdfs:label "phase mixin"@en ;
                   rdfs:seeAlso "https://ontouml.readthedocs.io/en/latest/classes/nonsortals/phasemixin/index.html"^^xsd:anyURI .


###  https://w3id.org/ontouml/2.0.0#quality
ontouml:quality rdf:type owl:NamedIndividual ,
                         ontouml:ClassStereotype ;
                rdfs:comment "A Quality is a particular type of intrinsic property that has a structured value. Qualities are things that existentially depend on the things they characterize, called their bearers."@en ;
                rdfs:isDefinedBy <https://w3id.org/ontouml/2.0.0> ;
                rdfs:label "quality"@en ;
                rdfs:seeAlso "https://ontouml.readthedocs.io/en/latest/classes/aspects/quality/index.html"^^xsd:anyURI .


###  https://w3id.org/ontouml/2.0.0#qualityNature
ontouml:qualityNature rdf:type owl:NamedIndividual ,
                               ontouml:OntologicalNature ;
                      rdfs:comment "Indicates that the restricted type includes quality individuals among its instances."@en ;
                      rdfs:isDefinedBy <https://w3id.org/ontouml/2.0.0> ;
                      rdfs:label "quality nature"@en .


###  https://w3id.org/ontouml/2.0.0#quantity
ontouml:quantity rdf:type owl:NamedIndividual ,
                          ontouml:ClassStereotype ;
                 rdfs:comment "Construct used to represent rigid concepts that provide an identity principle for their instances."@en ;
                 rdfs:isDefinedBy <https://w3id.org/ontouml/2.0.0> ;
                 rdfs:label "quantity"@en ;
                 rdfs:seeAlso "https://ontouml.readthedocs.io/en/latest/classes/sortals/quantity/index.html"^^xsd:anyURI .


###  https://w3id.org/ontouml/2.0.0#quantityNature
ontouml:quantityNature rdf:type owl:NamedIndividual ,
                                ontouml:OntologicalNature ;
                       rdfs:comment "Indicates that the restricted type includes quantity individuals among its instances."@en ;
                       rdfs:isDefinedBy <https://w3id.org/ontouml/2.0.0> ;
                       rdfs:label "quantity nature"@en .


###  https://w3id.org/ontouml/2.0.0#relator
ontouml:relator rdf:type owl:NamedIndividual ,
                         ontouml:ClassStereotype ;
                rdfs:comment "A construct used to represent truth-makers of material relations, i.e., the things that must exist for two or more individuals to be connected by material relations."@en ;
                rdfs:isDefinedBy <https://w3id.org/ontouml/2.0.0> ;
                rdfs:label "relator"@en ;
                rdfs:seeAlso "https://ontouml.readthedocs.io/en/latest/classes/sortals/relator/index.html"^^xsd:anyURI .


###  https://w3id.org/ontouml/2.0.0#relatorNature
ontouml:relatorNature rdf:type owl:NamedIndividual ,
                               ontouml:OntologicalNature ;
                      rdfs:comment "Indicates that the restricted type includes relator individuals among its instances."@en ;
                      rdfs:isDefinedBy <https://w3id.org/ontouml/2.0.0> ;
                      rdfs:label "relator nature"@en .


###  https://w3id.org/ontouml/2.0.0#role
ontouml:role rdf:type owl:NamedIndividual ,
                      ontouml:ClassStereotype ;
             rdfs:comment "Used to represent anti-rigid specializations of identity providers (Kind, Collective, Quantity, Relator, Mode, and Quantity) that are instantiated in relational contexts."@en ;
             rdfs:isDefinedBy <https://w3id.org/ontouml/2.0.0> ;
             rdfs:label "role"@en ;
             rdfs:seeAlso "https://ontouml.readthedocs.io/en/latest/classes/sortals/role/index.html"^^xsd:anyURI .


###  https://w3id.org/ontouml/2.0.0#roleMixin
ontouml:roleMixin rdf:type owl:NamedIndividual ,
                           ontouml:ClassStereotype ;
                  rdfs:comment "The equivalent of Role for types that aggregate instances with different identity principles."@en ;
                  rdfs:isDefinedBy <https://w3id.org/ontouml/2.0.0> ;
                  rdfs:label "role mixin"@en ;
                  rdfs:seeAlso "https://ontouml.readthedocs.io/en/latest/classes/nonsortals/rolemixin/index.html"^^xsd:anyURI .


###  https://w3id.org/ontouml/2.0.0#shared
ontouml:shared rdf:type owl:NamedIndividual ,
                        ontouml:AggregationKind ;
               rdfs:comment "Indicates that the ontouml:Property has shared aggregation semantics."@en ;
               rdfs:isDefinedBy <https://w3id.org/ontouml/2.0.0> ;
               rdfs:label "shared"@en .


###  https://w3id.org/ontouml/2.0.0#situation
ontouml:situation rdf:type owl:NamedIndividual ,
                           ontouml:ClassStereotype ;
                  rdfs:comment "Can be used to represent certain configurations of entities that can be comprehended as a whole."@en ;
                  rdfs:isDefinedBy <https://w3id.org/ontouml/2.0.0> ;
                  rdfs:label "situation"@en .


###  https://w3id.org/ontouml/2.0.0#situationNature
ontouml:situationNature rdf:type owl:NamedIndividual ,
                                 ontouml:OntologicalNature ;
                        rdfs:comment "Indicates that the restricted type includes situation individuals among its instances."@en ;
                        rdfs:isDefinedBy <https://w3id.org/ontouml/2.0.0> ;
                        rdfs:label "situation nature"@en .


###  https://w3id.org/ontouml/2.0.0#subCollectionOf
ontouml:subCollectionOf rdf:type owl:NamedIndividual ,
                                 ontouml:RelationStereotype ;
                        rdfs:comment "A parthood relation between two collectives."@en ;
                        rdfs:isDefinedBy <https://w3id.org/ontouml/2.0.0> ;
                        rdfs:label "sub collection of"@en ;
                        rdfs:seeAlso "https://ontouml.readthedocs.io/en/latest/relationships/aggregations/subCollectionOf/index.html"^^xsd:anyURI .


###  https://w3id.org/ontouml/2.0.0#subQuantityOf
ontouml:subQuantityOf rdf:type owl:NamedIndividual ,
                               ontouml:RelationStereotype ;
                      rdfs:comment "A parthood relation between two quantities."@en ;
                      rdfs:isDefinedBy <https://w3id.org/ontouml/2.0.0> ;
                      rdfs:label "sub quantity of"@en ;
                      rdfs:seeAlso "https://ontouml.readthedocs.io/en/latest/relationships/aggregations/subQuantityOf/index.html"^^xsd:anyURI .


###  https://w3id.org/ontouml/2.0.0#subkind
ontouml:subkind rdf:type owl:NamedIndividual ,
                         ontouml:ClassStereotype ;
                rdfs:comment "Used to represent rigid specializations of identity providers (Kind, Collective, Quantity, Relator, Mode, and Quantity)."@en ;
                rdfs:isDefinedBy <https://w3id.org/ontouml/2.0.0> ;
                rdfs:label "subkind"@en ;
                rdfs:seeAlso "https://ontouml.readthedocs.io/en/latest/classes/sortals/subkind/index.html"^^xsd:anyURI .


###  https://w3id.org/ontouml/2.0.0#termination
ontouml:termination rdf:type owl:NamedIndividual ,
                             ontouml:RelationStereotype ;
                    rdfs:comment "An individual of the ontouml:RelationStereotype used to assign the corresponding stereotype to a given ontouml:Relation."@en ;
                    rdfs:isDefinedBy <https://w3id.org/ontouml/2.0.0> ;
                    rdfs:label "termination"@en .


###  https://w3id.org/ontouml/2.0.0#triggers
ontouml:triggers rdf:type owl:NamedIndividual ,
                          ontouml:RelationStereotype ;
                 rdfs:comment "An individual of the ontouml:RelationStereotype used to assign the corresponding stereotype to a given ontouml:Relation."@en ;
                 rdfs:isDefinedBy <https://w3id.org/ontouml/2.0.0> ;
                 rdfs:label "triggers"@en .


###  https://w3id.org/ontouml/2.0.0#type
ontouml:type rdf:type owl:NamedIndividual ,
                      ontouml:ClassStereotype ;
             rdfs:comment "The stereotype for high-order types."@en ;
             rdfs:isDefinedBy <https://w3id.org/ontouml/2.0.0> ;
             rdfs:label "type"@en ;
             rdfs:seeAlso <https://doi.org/10.1007/978-3-031-17995-2_2> .


###  https://w3id.org/ontouml/2.0.0#typeNature
ontouml:typeNature rdf:type owl:NamedIndividual ,
                            ontouml:OntologicalNature ;
                   rdfs:comment "Indicates that the restricted type includes type individuals among its instances."@en ;
                   rdfs:isDefinedBy <https://w3id.org/ontouml/2.0.0> ;
                   rdfs:label "type nature"@en .


###  https://www.inf.unibz.it/krdb/
<https://www.inf.unibz.it/krdb/> rdf:type owl:NamedIndividual ,
                                          foaf:Organization ;
                                 foaf:homepage "https://www.inf.unibz.it/krdb/"^^xsd:anyURI ;
                                 foaf:member <https://orcid.org/0000-0003-3385-4769> ;
                                 foaf:name "KRDB Research Centre for Knowledge and Data, Free University of Bozen-Bolzano, Italy" .


###  https://www.utwente.nl/en/eemcs/scs/
<https://www.utwente.nl/en/eemcs/scs/> rdf:type owl:NamedIndividual ,
                                                foaf:Organization ;
                                       foaf:homepage "https://www.utwente.nl/en/eemcs/scs/"^^xsd:anyURI ;
                                       foaf:member <https://orcid.org/0000-0002-5385-5761> ,
                                                   <https://orcid.org/0000-0003-2528-3118> ,
                                                   <https://orcid.org/0000-0003-2736-7817> ;
                                       foaf:name "Semantics, Cybersecurity & Services (SCS), University of Twente, the Netherlands" .


#################################################################
#    Annotations
#################################################################

<https://orcid.org/0000-0002-5385-5761> foaf:name "Tiago Prince Sales" ;
                                        foaf:mbox "t.princesales@utwente.nl" .


<https://orcid.org/0000-0003-2528-3118> foaf:name "Claudenir M. Fonseca" ;
                                        foaf:mbox "c.moraisfonseca@utwente.nl" .


<https://orcid.org/0000-0003-2736-7817> foaf:name "Pedro Paulo Favato Barcelos" ;
                                        foaf:mbox "p.p.favatobarcelos@uwente.nl" .


<https://orcid.org/0000-0003-3385-4769> foaf:mbox "mattia.fumagalli@unibz.it" ;
                                        foaf:name "Mattia Fumagalli" .


#################################################################
#    General axioms
#################################################################

[ rdf:type owl:AllDisjointClasses ;
  owl:members ( ontouml:AggregationKind
                ontouml:Cardinality
                ontouml:OntologicalNature
                ontouml:OntoumlElement
                ontouml:Point
                ontouml:Stereotype
              )
] .


[ rdf:type owl:AllDifferent ;
  owl:distinctMembers ( <https://w3id.org/ontouml>
                        ontouml:abstract
                        ontouml:abstractNature
                        ontouml:begin
                        ontouml:bringsAbout
                        ontouml:category
                        ontouml:characterization
                        ontouml:collective
                        ontouml:collectiveNature
                        ontouml:comparative
                        ontouml:componentOf
                        ontouml:composite
                        ontouml:creation
                        ontouml:datatype
                        ontouml:derivation
                        ontouml:end
                        ontouml:enumeration
                        ontouml:event
                        ontouml:eventNature
                        ontouml:externalDependence
                        ontouml:extrinsicModeNature
                        ontouml:functionalComplexNature
                        ontouml:historicalDependence
                        ontouml:historicalRole
                        ontouml:historicalRoleMixin
                        ontouml:instantiation
                        ontouml:intrinsicModeNature
                        ontouml:kind
                        ontouml:manifestation
                        ontouml:material
                        ontouml:mediation
                        ontouml:memberOf
                        ontouml:mixin
                        ontouml:mode
                        ontouml:none
                        ontouml:participation
                        ontouml:participational
                        ontouml:phase
                        ontouml:phaseMixin
                        ontouml:quality
                        ontouml:qualityNature
                        ontouml:quantity
                        ontouml:quantityNature
                        ontouml:relator
                        ontouml:relatorNature
                        ontouml:role
                        ontouml:roleMixin
                        ontouml:shared
                        ontouml:situation
                        ontouml:situationNature
                        ontouml:subCollectionOf
                        ontouml:subQuantityOf
                        ontouml:subkind
                        ontouml:termination
                        ontouml:triggers
                        ontouml:type
                        ontouml:typeNature
                        <https://www.inf.unibz.it/krdb/>
                        <https://www.utwente.nl/en/eemcs/scs/>
                      )
] .


###  Generated by the OWL API (version 4.5.9.2019-02-01T07:24:44Z) https://github.com/owlcs/owlapi
