@prefix : <https://w3id.org/ontouml/2.0.0#> .
@prefix dct: <http://purl.org/dc/terms/> .
@prefix mod: <https://w3id.org/mod#> .
@prefix owl: <http://www.w3.org/2002/07/owl#> .
@prefix rdf: <http://www.w3.org/1999/02/22-rdf-syntax-ns#> .
@prefix xml: <http://www.w3.org/XML/1998/namespace> .
@prefix xsd: <http://www.w3.org/2001/XMLSchema#> .
@prefix dcat: <http://www.w3.org/ns/dcat#> .
@prefix foaf: <http://xmlns.com/foaf/0.1/> .
@prefix ocmv: <https://w3id.org/ontouml-models/vocabulary#> .
@prefix rdfs: <http://www.w3.org/2000/01/rdf-schema#> .
@prefix skos: <http://www.w3.org/2004/02/skos/core#> .
@prefix vann: <http://purl.org/vocab/vann/> .
@prefix ontouml: <https://w3id.org/ontouml/2.0.0#> .
@base <https://w3id.org/ontouml/2.0.0> .

<https://w3id.org/ontouml/2.0.0> rdf:type owl:Ontology ;
                                  owl:versionIRI <https://w3id.org/ontouml/vocabulary/v2.0.0> ;
                                  dct:conformsTo <https://w3id.org/ontouml/metamodel/v2.0.0> ;
                                  dct:contributor <https://orcid.org/0000-0003-3385-4769> ;
                                  dct:creator <https://orcid.org/0000-0002-5385-5761> ,
                                              <https://orcid.org/0000-0003-2528-3118> ,
                                              <https://orcid.org/0000-0003-2736-7817> ;
                                  dct:description "An OWL vocabulary to allow the serialization and exchanging of OntoUML models in conformance with the Ontouml Metamodel."@en ;
                                  dct:identifier "https://w3id.org/ontouml"^^xsd:anyURI ;
                                  dct:isReferencedBy <https://dblp.org/rec/conf/jowo/FonsecaSVFGA21.html> ,
                                                     <https://doi.org/10.1007/978-3-031-17995-2_1> ;
                                  dct:issued "2022-04-03"^^xsd:date ;
                                  dct:language <http://id.loc.gov/vocabulary/iso639-1/en> ;
                                  dct:license <https://creativecommons.org/licenses/by-sa/4.0> ;
                                  dct:modified "2023-08-14"^^xsd:date ;
                                  dct:publisher <https://www.utwente.nl/en/eemcs/scs/> ;
                                  dct:title "OntoUML Vocabulary"@en ;
                                  vann:preferredNamespacePrefix "ontouml" ;
                                  vann:preferredNamespaceUri "https://w3id.org/ontouml#"^^xsd:anyURI ;
                                  owl:priorVersion <https://w3id.org/ontouml/vocabulary/v1.1.0> ;
                                  owl:versionInfo "Release compatible with the OntoUML Metamodel 2.0.0."@en ;
                                  dcat:keyword "OntoUML"@en ,
                                               "OntoUML Metamodel"@en ,
                                               "Ontology-Driven Conceptual Modeling"@en ;
                                  dcat:landingPage <https://w3id.org/ontouml/vocabulary> ;
                                  foaf:homepage <https://w3id.org/ontouml/vocabulary/docs> .

#################################################################
#    Annotation properties
#################################################################

###  http://purl.org/dc/terms/conformsTo
dct:conformsTo rdf:type owl:AnnotationProperty .


###  http://purl.org/dc/terms/contributor
dct:contributor rdf:type owl:AnnotationProperty ;
                rdfs:range rdfs:Literal .


###  http://purl.org/dc/terms/creator
dct:creator rdf:type owl:AnnotationProperty ;
            rdfs:range rdfs:Literal .


###  http://purl.org/dc/terms/description
dct:description rdf:type owl:AnnotationProperty .


###  http://purl.org/dc/terms/identifier
dct:identifier rdf:type owl:AnnotationProperty .


###  http://purl.org/dc/terms/isReferencedBy
dct:isReferencedBy rdf:type owl:AnnotationProperty .


###  http://purl.org/dc/terms/issued
dct:issued rdf:type owl:AnnotationProperty .


###  http://purl.org/dc/terms/language
dct:language rdf:type owl:AnnotationProperty .


###  http://purl.org/dc/terms/license
dct:license rdf:type owl:AnnotationProperty .


###  http://purl.org/dc/terms/modified
dct:modified rdf:type owl:AnnotationProperty .


###  http://purl.org/dc/terms/publisher
dct:publisher rdf:type owl:AnnotationProperty ;
              rdfs:range rdfs:Literal .


###  http://purl.org/dc/terms/title
dct:title rdf:type owl:AnnotationProperty .


###  http://purl.org/vocab/vann/preferredNamespacePrefix
vann:preferredNamespacePrefix rdf:type owl:AnnotationProperty .


###  http://purl.org/vocab/vann/preferredNamespaceUri
vann:preferredNamespaceUri rdf:type owl:AnnotationProperty .


###  http://www.w3.org/ns/dcat#keyword
dcat:keyword rdf:type owl:AnnotationProperty .


###  http://www.w3.org/ns/dcat#landingPage
dcat:landingPage rdf:type owl:AnnotationProperty .


###  http://xmlns.com/foaf/0.1/homepage
foaf:homepage rdf:type owl:AnnotationProperty .


###  http://xmlns.com/foaf/0.1/mbox
foaf:mbox rdf:type owl:AnnotationProperty .


###  http://xmlns.com/foaf/0.1/member
foaf:member rdf:type owl:AnnotationProperty .


###  http://xmlns.com/foaf/0.1/name
foaf:name rdf:type owl:AnnotationProperty .


###  https://w3id.org/ontouml/2.0.0#description
ontouml:description rdf:type owl:AnnotationProperty ;
                    rdfs:subPropertyOf dct:description ;
                    rdfs:range rdfs:Literal ;
                    rdfs:domain ontouml:OntoumlElement .


###  https://w3id.org/ontouml/2.0.0#name
ontouml:name rdf:type owl:AnnotationProperty ;
             rdfs:subPropertyOf dct:title ;
             rdfs:range rdfs:Literal ;
             rdfs:domain ontouml:NamedElement .


#################################################################
#    Object Properties
#################################################################

###  http://purl.org/dc/terms/accessRights
dct:accessRights rdf:type owl:ObjectProperty ;
                 rdfs:comment "Identifies a dct:RightsStatement or a text concerning who and how the ontouml:Project can be accessed. E.g., the statement <http://publications.europa.eu/resource/authority/access-right/PUBLIC> informs that something is \"publicly accessible by everyone.\""@en ;
                 rdfs:isDefinedBy dct: ;
                 rdfs:label "access rights"@en .


###  http://purl.org/dc/terms/license
dct:license rdf:type owl:ObjectProperty .


###  http://purl.org/dc/terms/source
dct:source rdf:type owl:ObjectProperty ;
           rdfs:comment "Identifies a resource that contain, present, or significantly influenced the development of the ontouml:Project. We recommend the use of persistent and resolvable identifiers to refer to these resources, such as the Digital Object Identifier (DOI) or DBLP''s URI, such as, <https://doi.org/10.3233/AO-150150>, or <https://dblp.org/rec/journals/ao/Morales-Ramirez15>."@en ;
           rdfs:isDefinedBy dct: ;
           rdfs:label "source"@en .


###  http://www.w3.org/ns/dcat#landingPage
dcat:landingPage rdf:type owl:ObjectProperty .


###  http://www.w3.org/ns/dcat#theme
dcat:theme rdf:type owl:ObjectProperty ;
           rdfs:comment "Identifies a central theme of the ontouml:Project according to a theme taxonomy. In the OntoUML/UFO Catalog Metadata Vocabulary (OCMV), for example, the theme of an ontouml:Project must be a skos:Concept from the Library of Congress Classification (LCC), such as, \"Class S - Agriculture\", or \"Class T - Technology.\""@en ;
           rdfs:isDefinedBy <http://www.w3.org/ns/dcat> ;
           rdfs:label "theme"@en .


###  https://w3id.org/mod#designedForTask
mod:designedForTask rdf:type owl:ObjectProperty ;
                    rdfs:domain ontouml:SemanticArtefact ;
                    rdfs:range ontouml:SemanticArtefactTask ;
                    rdfs:comment """Identifies goals that motivated the development of the project. The OntoUML/UFO Catalog Metadata Vocabulary (OCMV) provides a list recurrent modeling goals for reuse:

- ocmv:ConceptualClarification: The project was created as the result of an ontological analysis of a concept, language, or domain of interest that sought to conceptually clarify and untangle complex notions and relations.

- ocmv:DataPublication: The project was created to support the publication of some datasets. For instance, a conceptual model used to generate an OWL vocabulary to publish tabular data as linked open data on the web.

- ocmv:DecisionSupportSystem: The project was created during the development of a decision support system.

- ocmv:Example: The project was created to demonstrate how OntoUML can be used to solve a certain modeling challenge, to support an experiment involving OntoUML, or to exemplify how a generic model can be reused in more concrete scenarios.

- ocmv:InformationRetrieval: The project was created to support the design of an information retrieval system.

- ocmv:Interoperability: The project was created to support data integration, vocabulary alignment, or the interoperability of software systems.

- ocmv:LanguageEngineering: The project was created for the design of a domain-specific modeling language.

- ocmv:Learning: The project was created so that its authors could learn UFO and OntoUML. This usually applies to models developed by students as part of their course assignments.

- ocmv:SoftwareEngineering: The project was created during the development of an information system. For instance, a conceptual model used to generate a relational database."""@en ;
                    rdfs:isDefinedBy <https://w3id.org/mod> ;
                    rdfs:label "designed for task"@en .


###  https://w3id.org/ontouml-models/vocabulary#context
ocmv:context rdf:type owl:ObjectProperty ;
             rdfs:comment """Identifies a context in which the ontouml:Project was developed. The OntoUML/UFO Catalog Metadata Vocabulary (OCMV) provides a set of recurrent modelling contexts:
          
- ocmv:Research: The project was developed as part of a research project. This usually implies that the project was featured in a scientific publication.

- ocmv:Industry: The project was developed for a public or private organization.

- ocmv:Classroom: The project was developed within the context of a course on conceptual modelling, most likely as a course assignment."""@en ;
             rdfs:isDefinedBy <https://w3id.org/ontouml-models/vocabulary> ;
             rdfs:label "context"@en .


###  https://w3id.org/ontouml-models/vocabulary#ontologyType
ocmv:ontologyType rdf:type owl:ObjectProperty ;
                  rdfs:comment """Identifies the classifications of the ontouml:Project according to its scope. The OntoUML/UFO Catalog Metadata Vocabulary (OCMV) provides a set of recurrent modelling scopes based on the work of Roussey et al. (2011):
          
- ocmv:Core: An ontology that grasps the central concepts and relations of a given domain, possibly integrating several domain ontologies and being applicable in multiple scenarios. E.g., UFO-S, a commitment-based ontology of services, can be considered a core ontology because it applies to services in multiple domains, such as medical, financial, and legal services.

- ocmv:Domain: An ontology that describes how a community conceptualizes a phenomenon of interest. In general, a domain ontology formally characterizes a much narrower domain than a core ontology does. E.g., OntoBio is a domain ontology of biodiversity.

- ocmv:Application: An ontology that specializes a domain ontology where there could be no consensus or knowledge sharing. It represents the particular model of a domain according to a single viewpoint of a user or a developer."""@en ;
                  rdfs:isDefinedBy <https://w3id.org/ontouml-models/vocabulary> ;
                  rdfs:label "ontology type"@en .


###  https://w3id.org/ontouml-models/vocabulary#representationStyle
ocmv:representationStyle rdf:type owl:ObjectProperty ;
                         rdfs:comment """Identifies the representation style adopted in the ontouml:Project between \"OntoUML Style\" and \"UFO Style\":
          
- ocmv:OntoumlStyle: Characterizes a project that contains at least one class, relation, or property using a valid OntoUML stereotype.

- ocmv:UfoStyle: Characterizes a project that contains at least one class or relation from UFO without an OntoUML stereotype."""@en ;
                         rdfs:isDefinedBy <https://w3id.org/ontouml-models/vocabulary> ;
                         rdfs:label "representation style"@en .


###  https://w3id.org/ontouml/2.0.0#aggregationKind
ontouml:aggregationKind rdf:type owl:ObjectProperty ;
                        rdfs:domain ontouml:Property ;
                        rdfs:range ontouml:AggregationKind ;
                        rdfs:comment """Identifies the ontouml:AggregationKind of an ontouml:Property (a relation end) as a whole in a parthood (mereological) relation.

Examples include \"Project Member\" as a \"shared\" part of a \"Project Team\" and an \"Engine\" as a \"composite\" part of a \"Vehicle.\"

The possible values for aggregation kind are ontouml:composite (when parts are exclusive to one whole), ontouml:shared (when parts can be shared), and ontouml:none (for non-parthood relations)."""@en ;
                        rdfs:isDefinedBy <https://w3id.org/ontouml/2.0.0> ;
                        rdfs:label "aggregation kind"@en .


###  https://w3id.org/ontouml/2.0.0#attribute
ontouml:attribute rdf:type owl:ObjectProperty ;
                  rdfs:subPropertyOf ontouml:property ;
                  rdfs:domain ontouml:Class ;
                  rdfs:range ontouml:Property ;
                  rdfs:comment "Relates an instance of an ontouml:Class to its properties, which are instances of the ontouml:Property class."@en ;
                  rdfs:isDefinedBy <https://w3id.org/ontouml/2.0.0> ;
                  rdfs:label "attribute"@en .


###  https://w3id.org/ontouml/2.0.0#cardinality
ontouml:cardinality rdf:type owl:ObjectProperty ;
                    rdfs:domain ontouml:Property ;
                    rdfs:range ontouml:Cardinality ;
                    rdfs:comment "Identifies the individual of type ontouml:Cardinality that represents the cardinalities of an ontouml:Property."@en ;
                    rdfs:isDefinedBy <https://w3id.org/ontouml/2.0.0> ;
                    rdfs:label "cardinality"@en .


###  https://w3id.org/ontouml/2.0.0#categorizer
ontouml:categorizer rdf:type owl:ObjectProperty ;
                    rdfs:domain ontouml:GeneralizationSet ;
                    rdfs:range ontouml:Class ;
                    rdfs:comment """Identifies the high-order ontouml:Class that classifies (i.e., is instantiated by) every specific ontouml:Class in the ontouml:GeneralizationSet.

For example, \"Academic Role\" as the categorizer of the generalization set of \"Person\" into \"Student\" and \"Teacher\" representing the specific classes as instances of the categorizer.

A categorizer can only be present in generalization sets involving exclusively classes."""@en ;
                    rdfs:isDefinedBy <https://w3id.org/ontouml/2.0.0> ;
                    rdfs:label "categorizer"@en ;
                    rdfs:seeAlso <https://doi.org/10.1007/978-3-031-17995-2_2> ,
                                 <https://doi.org/10.1016/j.datak.2022.102012> .


###  https://w3id.org/ontouml/2.0.0#containsModelElement
ontouml:containsModelElement rdf:type owl:ObjectProperty ;
                             rdfs:domain ontouml:Package ;
                             rdfs:range ontouml:PackageableElement ;
                             rdfs:comment "Identifies an ontouml:PackageableElement that is a content of an ontouml:Package."@en ;
                             rdfs:isDefinedBy <https://w3id.org/ontouml/2.0.0> ;
                             rdfs:label "contains model element"@en .


###  https://w3id.org/ontouml/2.0.0#containsView
ontouml:containsView rdf:type owl:ObjectProperty ;
                     rdfs:domain ontouml:Diagram ;
                     rdfs:range ontouml:View ;
                     rdfs:comment "Identifies an ontouml:View contained in the ontouml:Diagram."@en ;
                     rdfs:isDefinedBy <https://w3id.org/ontouml/2.0.0> ;
                     rdfs:label "contains view"@en .


###  https://w3id.org/ontouml/2.0.0#diagram
ontouml:diagram rdf:type owl:ObjectProperty ;
                rdfs:domain ontouml:Project ;
                rdfs:range ontouml:Diagram ;
                rdfs:comment "Identifies which entities of type ontouml:Diagram are part of an ontouml:Project."@en ,
                             "It is mapped to the OntoUML Metamodel's 'diagrams' relation between the Project and Diagram classes."@en ;
                rdfs:isDefinedBy <https://w3id.org/ontouml/2.0.0> ;
                rdfs:label "diagram"@en .


###  https://w3id.org/ontouml/2.0.0#element
ontouml:element rdf:type owl:ObjectProperty ;
                owl:inverseOf ontouml:project ;
                rdfs:domain ontouml:Project ;
                rdfs:range [ rdf:type owl:Class ;
                             owl:unionOf ( ontouml:Diagram
                                           ontouml:PackageableElement
                                           ontouml:View
                                         )
                           ] ;
                rdfs:comment "Identifies the ontouml:Diagram, ontouml:PackageableElement, or ontouml:View elements that is contained in the ontouml:Project."@en ;
                rdfs:isDefinedBy <https://w3id.org/ontouml/2.0.0> ;
                rdfs:label "element"@en .


###  https://w3id.org/ontouml/2.0.0#general
ontouml:general rdf:type owl:ObjectProperty ;
                rdfs:domain ontouml:Generalization ;
                rdfs:range ontouml:Classifier ;
                rdfs:comment "Identifies the general ontouml:Classifier of an ontouml:Generalization element. E.g., in the generalization of \"Student\" into \"Person\", \"Person\" is the general classifier."@en ;
                rdfs:isDefinedBy <https://w3id.org/ontouml/2.0.0> ;
                rdfs:label "general"@en .


###  https://w3id.org/ontouml/2.0.0#generalization
ontouml:generalization rdf:type owl:ObjectProperty ;
                       rdfs:domain ontouml:GeneralizationSet ;
                       rdfs:range ontouml:Generalization ;
                       rdfs:comment "Identifies a ontouml:Generalization element that is involved in an ontouml:GeneralizationSet."@en ;
                       rdfs:isDefinedBy <https://w3id.org/ontouml/2.0.0> ;
                       rdfs:label "generalization"@en .


###  https://w3id.org/ontouml/2.0.0#isViewOf
ontouml:isViewOf rdf:type owl:ObjectProperty ;
                 rdfs:domain ontouml:View ;
                 rdfs:range ontouml:ModelElement ;
                 rdfs:comment "Identifies the ontouml:ModelElement that the ontouml:View represents in the ontouml:Diagram."@en ;
                 rdfs:isDefinedBy <https://w3id.org/ontouml/2.0.0> ;
                 rdfs:label "is view of"@en .


###  https://w3id.org/ontouml/2.0.0#linkedElement
ontouml:linkedElement rdf:type owl:ObjectProperty ;
                      rdfs:domain ontouml:Link ;
                      rdfs:range ontouml:ModelElement ;
                      rdfs:comment "Identifies the ontouml:ModelElement the ontouml:Link connects."@en ;
                      rdfs:isDefinedBy <https://w3id.org/ontouml/2.0.0> ;
                      rdfs:label "linked element"@en .


###  https://w3id.org/ontouml/2.0.0#linkedNote
ontouml:linkedNote rdf:type owl:ObjectProperty ;
                   rdfs:domain ontouml:Link ;
                   rdfs:range ontouml:Note ;
                   rdfs:comment "Identifies the ontouml:Note the ontouml:Link connects."@en ;
                   rdfs:isDefinedBy <https://w3id.org/ontouml/2.0.0> ;
                   rdfs:label "linked note"@en .


###  https://w3id.org/ontouml/2.0.0#literal
ontouml:literal rdf:type owl:ObjectProperty ;
                rdfs:domain ontouml:Class ;
                rdfs:range ontouml:Literal ;
                rdfs:comment "Identifies an ontouml:Literal of an ontouml:Class decorated with the ontouml:Stereotype ontouml:enumeration."@en ;
                rdfs:isDefinedBy <https://w3id.org/ontouml/2.0.0> ;
                rdfs:label "literal"@en .


###  https://w3id.org/ontouml/2.0.0#model
ontouml:model rdf:type owl:ObjectProperty ;
              rdfs:domain ontouml:Project ;
              rdfs:range ontouml:Package ;
              rdfs:comment "Relates an ontouml:Project to an ontouml:Package that is part of it."@en ;
              rdfs:isDefinedBy <https://w3id.org/ontouml/2.0.0> ;
              rdfs:label "model"@en .


###  https://w3id.org/ontouml/2.0.0#owner
ontouml:owner rdf:type owl:ObjectProperty ;
              rdfs:domain ontouml:Diagram ;
              rdfs:range ontouml:ModelElement ;
              rdfs:comment "Identifies the ontouml:ModelElement that is the owner of the ontouml:Diagram."@en ;
              rdfs:isDefinedBy <https://w3id.org/ontouml/2.0.0> ;
              rdfs:label "owner"@en .


###  https://w3id.org/ontouml/2.0.0#point
ontouml:point rdf:type owl:ObjectProperty ;
              rdfs:domain ontouml:Path ;
              rdfs:range ontouml:Point ;
              rdfs:comment "Relates an ontouml:Path to an ontouml:Point that composes it."@en ;
              rdfs:isDefinedBy <https://w3id.org/ontouml/2.0.0> ;
              rdfs:label "point"@en .


###  https://w3id.org/ontouml/2.0.0#project
ontouml:project rdf:type owl:ObjectProperty ;
                rdfs:range ontouml:Project ;
                rdfs:comment "Relates an ontouml:OntoumlElement different than ontouml:Project to an ontouml:Project that it composes."@en ;
                rdfs:isDefinedBy <https://w3id.org/ontouml/2.0.0> ;
                rdfs:label "project"@en .


###  https://w3id.org/ontouml/2.0.0#property
ontouml:property rdf:type owl:ObjectProperty ;
                 rdfs:domain ontouml:Classifier ;
                 rdfs:range ontouml:Property ;
                 rdfs:comment "Identifies the properties contained in a classifier. These properties are referred to as attributes, when contained by classes, and relation ends, when contained by relations."@en ;
                 rdfs:isDefinedBy <https://w3id.org/ontouml/2.0.0> ;
                 rdfs:label "property"@en .


###  https://w3id.org/ontouml/2.0.0#propertyType
ontouml:propertyType rdf:type owl:ObjectProperty ;
                     rdfs:domain ontouml:Property ;
                     rdfs:range ontouml:Classifier ;
                     rdfs:comment "Identifies the ontouml:Classifier instantiated by the values assigned to the ontouml:Property."@en ;
                     rdfs:isDefinedBy <https://w3id.org/ontouml/2.0.0> ;
                     rdfs:label "property type"@en .


###  https://w3id.org/ontouml/2.0.0#redefinesProperty
ontouml:redefinesProperty rdf:type owl:ObjectProperty ;
                          rdfs:domain ontouml:Property ;
                          rdfs:range ontouml:Property ;
                          rdfs:comment """Identifies the relation end (an ontouml:Property) that provides redefinition constraints to the ontouml:Property.

Examples include, in the relations (i) \"works in\" from \"Project Member\" to \"Project\", and (ii) \"leads\" from \"Project Leader\" to \"Project\", where the member end is redefined for the leader who can only be connected to the project through that specific relation.

Redefinition can only occur on the relation ends when both sides of the involved relations are connected to the same classifiers or classifiers that are in the same generalization chain."""@en ;
                          rdfs:isDefinedBy <https://w3id.org/ontouml/2.0.0> ;
                          rdfs:label "redefines property"@en ;
                          rdfs:seeAlso <https://doi.org/10.1007/978-3-642-24606-7_15> .


###  https://w3id.org/ontouml/2.0.0#relationEnd
ontouml:relationEnd rdf:type owl:ObjectProperty ;
                    rdfs:subPropertyOf ontouml:property ;
                    rdfs:domain ontouml:Relation ;
                    rdfs:range ontouml:Property ;
                    rdfs:comment "Identifies a property that represents one end (source or target) of an ontouml:Relation."@en ;
                    rdfs:isDefinedBy <https://w3id.org/ontouml/2.0.0> ;
                    rdfs:label "relation end"@en .


###  https://w3id.org/ontouml/2.0.0#restrictedTo
ontouml:restrictedTo rdf:type owl:ObjectProperty ;
                     rdfs:domain ontouml:Class ;
                     rdfs:range ontouml:OntologicalNature ;
                     rdfs:comment """Identifies a possible ontouml:OntologicalNature for the instances of an ontouml:Class.

Examples include the class \"Vehicle\" restricted to having \"functional-complex\" instances, and the class \"Insured Item\" restricted to \"functional-complex\" and \"relator\" (e.g., employment insurance)."""@en ;
                     rdfs:isDefinedBy <https://w3id.org/ontouml/2.0.0> ;
                     rdfs:label "restricted to"@en .


###  https://w3id.org/ontouml/2.0.0#root
ontouml:root rdf:type owl:ObjectProperty ;
             rdfs:domain ontouml:Project ;
             rdfs:range ontouml:Package ;
             rdfs:comment "Identifies the root ontouml:Package of an ontouml:Project (the package containing all other model elements of the project) if present."@en ;
             rdfs:isDefinedBy <https://w3id.org/ontouml/2.0.0> ;
             rdfs:label "root"@en .


###  https://w3id.org/ontouml/2.0.0#shape
ontouml:shape rdf:type owl:ObjectProperty ;
              rdfs:domain ontouml:View ;
              rdfs:range ontouml:Shape ;
              rdfs:comment "Relates an ontouml:ElementView to an ontouml:Shape that contains the diagramation's data (size and position) about the ontouml:ModelElement it is a view of."@en ;
              rdfs:isDefinedBy <https://w3id.org/ontouml/2.0.0> ;
              rdfs:label "shape"@en .


###  https://w3id.org/ontouml/2.0.0#sourceEnd
ontouml:sourceEnd rdf:type owl:ObjectProperty ;
                  rdfs:subPropertyOf ontouml:relationEnd ;
                  rdfs:domain ontouml:Relation ;
                  rdfs:range ontouml:Property ;
                  rdfs:comment "Identifies an ontouml:Property that represents the source side of an ontouml:Relation."@en ;
                  rdfs:isDefinedBy <https://w3id.org/ontouml/2.0.0> ;
                  rdfs:label "source end"@en .


###  https://w3id.org/ontouml/2.0.0#sourceView
ontouml:sourceView rdf:type owl:ObjectProperty ;
                   rdfs:domain ontouml:BinaryConnectorView ;
                   rdfs:range ontouml:View ;
                   rdfs:comment "Identifies an ontouml:ElementView that participates as source of an ontouml:RelationView or ontouml:GeneralizationView."@en ;
                   rdfs:isDefinedBy <https://w3id.org/ontouml/2.0.0> ;
                   rdfs:label "source view"@en .


###  https://w3id.org/ontouml/2.0.0#specific
ontouml:specific rdf:type owl:ObjectProperty ;
                 rdfs:domain ontouml:Generalization ;
                 rdfs:range ontouml:Classifier ;
                 rdfs:comment "Identifies the specific ontouml:Classifier of an ontouml:Generalization element. E.g., in the generalization of \"Student\" into \"Person\", \"Student\" is the specific classifier."@en ;
                 rdfs:isDefinedBy <https://w3id.org/ontouml/2.0.0> ;
                 rdfs:label "specific"@en .


###  https://w3id.org/ontouml/2.0.0#stereotype
ontouml:stereotype rdf:type owl:ObjectProperty ;
                   rdfs:domain ontouml:DecoratableElement ;
                   rdfs:range ontouml:Stereotype ;
                   rdfs:comment "Identifies the type of an ontouml:DecoratableElement according to Unified Foundational Ontology (UFO)."@en ;
                   rdfs:isDefinedBy <https://w3id.org/ontouml/2.0.0> ;
                   rdfs:label "stereotype"@en .


###  https://w3id.org/ontouml/2.0.0#subsetsProperty
ontouml:subsetsProperty rdf:type owl:ObjectProperty ;
                        rdfs:domain ontouml:Property ;
                        rdfs:range ontouml:Property ;
                        rdfs:comment """Identifies the relation end (an ontouml:Property) that provides subsetting constraints to the ontouml:Property.

Examples include, in the relations (i) \"works for\" from \"Employee\" to \"Organization\", and (ii) \"teaches for\" from \"Teacher\" to \"University\", both relation ends of (ii) are subsets of their respect ends in (i).

Subsetting can only occur on the relation ends when both sides of the involved relations are connected to the same classifiers or classifiers that are in the same generalization chain.

Subsetting can also be represented through a generalization between relations."""@en ;
                        rdfs:isDefinedBy <https://w3id.org/ontouml/2.0.0> ;
                        rdfs:label "subsets property"@en ;
                        rdfs:seeAlso <https://doi.org/10.1007/978-3-642-24606-7_15> .


###  https://w3id.org/ontouml/2.0.0#targetEnd
ontouml:targetEnd rdf:type owl:ObjectProperty ;
                  rdfs:subPropertyOf ontouml:relationEnd ;
                  rdfs:domain ontouml:Relation ;
                  rdfs:range ontouml:Property ;
                  rdfs:comment "Identifies an ontouml:Property that represents the target side of an ontouml:Relation."@en ;
                  rdfs:isDefinedBy <https://w3id.org/ontouml/2.0.0> ;
                  rdfs:label "target end"@en .


###  https://w3id.org/ontouml/2.0.0#targetView
ontouml:targetView rdf:type owl:ObjectProperty ;
                   rdfs:domain ontouml:BinaryConnectorView ;
                   rdfs:range ontouml:View ;
                   rdfs:comment "Identifies an ontouml:ElementView that participates as target of an ontouml:ConnectorView."@en ;
                   rdfs:isDefinedBy <https://w3id.org/ontouml/2.0.0> ;
                   rdfs:label "target view"@en .


###  https://w3id.org/ontouml/2.0.0#topLeftPosition
ontouml:topLeftPosition rdf:type owl:ObjectProperty ;
                        rdfs:domain ontouml:RectangularShape ;
                        rdfs:range ontouml:Point ;
                        rdfs:comment "Is direct mapped to the OntoUML Metamodel's 'topLeft' relationship between the classes RectangularShape and Point."@en ,
                                     "Relates an ontouml:RectangularShape to an ontouml:Point that contains the horizontal and vertical coordinates (ontouml:xCoordinate and ontouml:yCoordinate, respectively) representing the former's top left position in an ontouml:Diagram."@en ;
                        rdfs:isDefinedBy <https://w3id.org/ontouml/2.0.0> ;
                        rdfs:label "top left position"@en .


#################################################################
#    Data properties
#################################################################

###  http://purl.org/dc/terms/alternative
dct:alternative rdf:type owl:DatatypeProperty ;
                rdfs:range rdfs:Literal ;
                rdfs:comment "Determines a dct:alternative name of the ontouml:NamedElement using a rdf:langString. Alternative names are not translations names, but indeed alternatives or synonyms to the name."@en ;
                rdfs:isDefinedBy dct: ;
                rdfs:label "alternative"@en .


###  http://purl.org/dc/terms/bibliographicCitation
dct:bibliographicCitation rdf:type owl:DatatypeProperty ;
                          rdfs:comment "Determines a bibliographic reference for the ontouml:Project using a xsd:string or an rdf:langString literal. E.g., \"Weigand, H., Johannesson, P., & Andersson, B. (2021). An artifact ontology for design science research. Data & Knowledge Engineering, 133\"@en."@en ;
                          rdfs:isDefinedBy dct: ;
                          rdfs:label "bibliographic citation"@en .


###  http://purl.org/dc/terms/contributor
dct:contributor rdf:type owl:DatatypeProperty .


###  http://purl.org/dc/terms/creator
dct:creator rdf:type owl:DatatypeProperty .


###  http://purl.org/dc/terms/language
dct:language rdf:type owl:DatatypeProperty .


###  http://purl.org/dc/terms/publisher
dct:publisher rdf:type owl:DatatypeProperty .


###  http://www.w3.org/2004/02/skos/core#editorialNote
skos:editorialNote rdf:type owl:DatatypeProperty ;
                   rdfs:range rdfs:Literal ;
                   rdfs:comment "Determines a general note about the ontouml:NamedElement using an array of language strings. Editorial notes are typically notes on the development process and must not be confused with descriptions."@en ;
                   rdfs:isDefinedBy <http://www.w3.org/2004/02/skos/core> ;
                   rdfs:label "editorial note"@en .


###  http://www.w3.org/ns/dcat#keyword
dcat:keyword rdf:type owl:DatatypeProperty .


###  https://w3id.org/mod#acronym
mod:acronym rdf:type owl:DatatypeProperty ;
            rdfs:domain ontouml:SemanticArtefact ;
            rdfs:range xsd:string ;
            rdfs:comment "Determines an acronym one can use to refer to the ontouml:Project using xsd:string literals. E.g., \"RDBS-O\", \"COVER\", \"ROT.\""@en ;
            rdfs:isDefinedBy <https://w3id.org/mod> ;
            rdfs:label "acronym"@en .


###  https://w3id.org/ontouml/2.0.0#cardinalityValue
ontouml:cardinalityValue rdf:type owl:DatatypeProperty ;
                         rdfs:domain ontouml:Cardinality ;
                         rdfs:range xsd:string ;
                         rdfs:comment """Determines the value of an ontouml:Cardinality using a string. 

Examples include \"Person\" with cardinality \"1\" (exactly one) in the property (attribute) \"name\", and cardinality \"0..*\" (zero or more) in the property (related end) \"friends\" of the relation \"friends with\".

The cardinality should follow the regular express \"^\\d+(\\.\\.(\\d+|\\*))?$\", where the number before \"..\" represents the lower bound, the number or \"*\" after represent the upper bound. In case the \"..\" is not present, a number represents an exact number of instances, and \"*\" represents \"zero or more\" instances.

This regular expression is not enforced to accommodate theoretical ranges as expression, such as, \"a..b\"."""@en ;
                         rdfs:isDefinedBy <https://w3id.org/ontouml/2.0.0> ;
                         rdfs:label "cardinality value"@en .


###  https://w3id.org/ontouml/2.0.0#description
ontouml:description rdf:type owl:DatatypeProperty .


###  https://w3id.org/ontouml/2.0.0#height
ontouml:height rdf:type owl:DatatypeProperty ;
               rdfs:domain ontouml:RectangularShape ;
               rdfs:range xsd:positiveInteger ;
               rdfs:comment "Indicates the height of an ontouml:RectangularShape that is represented in an ontouml:Diagram."@en ;
               rdfs:isDefinedBy <https://w3id.org/ontouml/2.0.0> ;
               rdfs:label "height"@en .


###  https://w3id.org/ontouml/2.0.0#isAbstract
ontouml:isAbstract rdf:type owl:DatatypeProperty ;
                   rdfs:domain ontouml:Classifier ;
                   rdfs:range xsd:boolean ;
                   rdfs:comment "Determines whether the ontouml:Classifier can have direct instances using a xsd:boolean. Abstract classifiers can only have instances when these are also instances of some other classifier that is not abstract (i.e., concrete) and is a specialization of the abstract one."@en ;
                   rdfs:isDefinedBy <https://w3id.org/ontouml/2.0.0> ;
                   rdfs:label "is abstract"@en .


###  https://w3id.org/ontouml/2.0.0#isComplete
ontouml:isComplete rdf:type owl:DatatypeProperty ;
                   rdfs:domain ontouml:GeneralizationSet ;
                   rdfs:range xsd:boolean ;
                   rdfs:comment """Determines whether the specific ontouml:Classifier elements in the ontouml:GeneralizationSet completely cover the extension of the general ontouml:Classifier.

Examples include the generalization set involving \"Child\" and \"Adult\" generalized into \"Person\", where the \"is complete\" as \"true\" indicates that every person is either an instance of \"Child\" or \"Adult.\""""@en ;
                   rdfs:isDefinedBy <https://w3id.org/ontouml/2.0.0> ;
                   rdfs:label "is complete"@en .


###  https://w3id.org/ontouml/2.0.0#isDerived
ontouml:isDerived rdf:type owl:DatatypeProperty ;
                  rdfs:domain ontouml:DecoratableElement ;
                  rdfs:range xsd:boolean ;
                  rdfs:comment """Determines whether the ontouml:DecoratableElement is derived from a different ontouml:ModelElement, i.e., whether a different ontouml:ModelElement serves as its truthmaker.

Examples include the comparative relation \"is heavier than\" between two physical objects which is derived from their \"Weight\" quality."""@en ;
                  rdfs:isDefinedBy <https://w3id.org/ontouml/2.0.0> ;
                  rdfs:label "is derived"@en ;
                  rdfs:seeAlso <https://doi.org/10.1007/978-3-030-00847-5_13> ,
                               <https://doi.org/10.1007/978-3-030-33223-5_4> .


###  https://w3id.org/ontouml/2.0.0#isDisjoint
ontouml:isDisjoint rdf:type owl:DatatypeProperty ;
                   rdfs:domain ontouml:GeneralizationSet ;
                   rdfs:range xsd:boolean ;
                   rdfs:comment """Determines whether the specific ontouml:Classifier elements in the ontouml:GeneralizationSet have disjoint extensions.

Examples include the generalization set involving \"Child\" and \"Adult\" generalized into \"Person\", where the \"is disjoint\" as \"true\" indicates that no person is simultaneously instance of \"Child\" and \"Adult.\""""@en ;
                   rdfs:isDefinedBy <https://w3id.org/ontouml/2.0.0> ;
                   rdfs:label "is disjoint"@en .


###  https://w3id.org/ontouml/2.0.0#isExtensional
ontouml:isExtensional rdf:type owl:DatatypeProperty ;
                      rdfs:domain ontouml:Class ;
                      rdfs:range xsd:boolean ;
                      rdfs:comment "Indicates if an ontouml:Class is extensionally defined (i.e., it's parts cannot change)."@en ;
                      rdfs:isDefinedBy <https://w3id.org/ontouml/2.0.0> ;
                      rdfs:label "is extensional"@en .


###  https://w3id.org/ontouml/2.0.0#isOrdered
ontouml:isOrdered rdf:type owl:DatatypeProperty ;
                  rdfs:domain ontouml:Property ;
                  rdfs:range xsd:boolean ;
                  rdfs:comment "Determines whether the order of assignments of a property carries meaning using a xsd:boolean. This boolean only regards properties whose maximum cardinality greater than one."@en ;
                  rdfs:isDefinedBy <https://w3id.org/ontouml/2.0.0> ;
                  rdfs:label "is ordered"@en .


###  https://w3id.org/ontouml/2.0.0#isPowertype
ontouml:isPowertype rdf:type owl:DatatypeProperty ;
                    rdfs:domain ontouml:Class ;
                    rdfs:range xsd:boolean ;
                    rdfs:comment "Determines whether the high-order ontouml:Class is a \"Cardelli powertype\" using a xsd:boolean. In other words, determines whether the high-order class is defined as the one whose instances are its base type plus all possible specializations of it."@en ;
                    rdfs:isDefinedBy <https://w3id.org/ontouml/2.0.0> ;
                    rdfs:label "is powertype"@en ;
                    rdfs:seeAlso <https://doi.org/10.1007/978-3-031-17995-2_2> .


###  https://w3id.org/ontouml/2.0.0#isReadOnly
ontouml:isReadOnly rdf:type owl:DatatypeProperty ;
                   rdfs:domain ontouml:Property ;
                   rdfs:range xsd:boolean ;
                   rdfs:comment "Determines whether the assignments of an ontouml:Property are immutable using a xsd:boolean."@en ;
                   rdfs:isDefinedBy <https://w3id.org/ontouml/2.0.0> ;
                   rdfs:label "is read only"@en .


###  https://w3id.org/ontouml/2.0.0#lowerBound
ontouml:lowerBound rdf:type owl:DatatypeProperty ;
                   rdfs:domain ontouml:Cardinality ;
                   rdfs:range xsd:nonNegativeInteger ;
                   rdfs:comment "An ontouml:Cardinality's lower bound must correspond to the one indicated by its ontouml:cardinalityValue property." ,
                                "E.g., if the ontouml:cardinalityValue set is [1..*] then the lower bound is '1'."@en ,
                                "Identifies the lower bound of an ontouml:Cardinality."@en ;
                   rdfs:isDefinedBy <https://w3id.org/ontouml/2.0.0> ;
                   rdfs:label "lower bound"@en .


###  https://w3id.org/ontouml/2.0.0#name
ontouml:name rdf:type owl:DatatypeProperty .


###  https://w3id.org/ontouml/2.0.0#namespace
ontouml:namespace rdf:type owl:DatatypeProperty ;
                  rdfs:domain ontouml:Project ;
                  rdfs:range xsd:anyURI ;
                  rdfs:comment "Determines the namespace (or \"base prefix\") for every ontouml:OntoumlElement in the ontouml:Project using a xsd:anyURI string. When present, the namespace should be the URI prefix of all elements in the project forming a globally unique resolvable URI for identification in the web as a FAIR Digital Object."@en ;
                  rdfs:isDefinedBy <https://w3id.org/ontouml/2.0.0> ;
                  rdfs:label "namespace"@en .


###  https://w3id.org/ontouml/2.0.0#order
ontouml:order rdf:type owl:DatatypeProperty ;
              rdfs:domain ontouml:Class ;
              rdfs:range xsd:string ;
              rdfs:comment "Determines the instantiation order of an ontouml:Class using a string. Examples include ordered classes such as first-order classes (order \"1\"), second-order classes (order \"2\"), and third-order classes (order \"3\"), and orderless classes (order \"*\")."@en ;
              rdfs:isDefinedBy <https://w3id.org/ontouml/2.0.0> ;
              rdfs:label "order"@en ;
              rdfs:seeAlso <https://doi.org/10.1007/978-3-031-17995-2_2> .


###  https://w3id.org/ontouml/2.0.0#text
ontouml:text rdf:type owl:DatatypeProperty ;
             rdfs:domain ontouml:Note ;
             rdfs:range rdfs:Literal ;
             rdfs:comment "Determines the contents of an ontouml:Note using a xsd:string or an rdf:langString literal."@en ;
             rdfs:isDefinedBy <https://w3id.org/ontouml/2.0.0> ;
             rdfs:label "text"@en .


###  https://w3id.org/ontouml/2.0.0#upperBound
ontouml:upperBound rdf:type owl:DatatypeProperty ;
                   rdfs:domain ontouml:Cardinality ;
                   rdfs:range rdfs:Literal ;
                   rdfs:comment "An ontouml:Cardinality's upper bound must correspond to the one indicated by its ontouml:cardinalityValue property." ,
                                "E.g., if the ontouml:cardinalityValue set is [1..*] then the upper bound is '*'."@en ,
                                "Identifies the upper bound of an ontouml:Cardinality."@en ;
                   rdfs:isDefinedBy <https://w3id.org/ontouml/2.0.0> ;
                   rdfs:label "upper bound"@en .


###  https://w3id.org/ontouml/2.0.0#width
ontouml:width rdf:type owl:DatatypeProperty ;
              rdfs:domain ontouml:RectangularShape ;
              rdfs:range xsd:positiveInteger ;
              rdfs:comment "Indicates the width of an ontouml:RectangularShape that is represented in an ontouml:Diagram."@en ;
              rdfs:isDefinedBy <https://w3id.org/ontouml/2.0.0> ;
              rdfs:label "width"@en .


###  https://w3id.org/ontouml/2.0.0#xCoordinate
ontouml:xCoordinate rdf:type owl:DatatypeProperty ;
                    rdfs:domain ontouml:Point ;
                    rdfs:range xsd:integer ;
                    rdfs:comment "Is direct mapped to the metamodel's 'x' attribute of the Point class."@en ,
                                 "Relates an ontouml:Point to the value indicating the specific x (horizontal) coordinate of the top left position of an ontouml:RectangularShape."@en ;
                    rdfs:isDefinedBy <https://w3id.org/ontouml/2.0.0> ;
                    rdfs:label "x-coordinate"@en .


###  https://w3id.org/ontouml/2.0.0#yCoordinate
ontouml:yCoordinate rdf:type owl:DatatypeProperty ;
                    rdfs:domain ontouml:Point ;
                    rdfs:range xsd:integer ;
                    rdfs:comment "Is direct mapped to the metamodel's 'y' attribute of the Point class."@en ,
                                 "Relates an ontouml:Point to the value indicating the specific y (vertical) coordinate of the top left position of an ontouml:RectangularShape."@en ;
                    rdfs:isDefinedBy <https://w3id.org/ontouml/2.0.0> ;
                    rdfs:label "y-coordinate"@en .


#################################################################
#    Classes
#################################################################

###  http://purl.org/dc/terms/Standard
dct:Standard rdf:type owl:Class .


###  http://xmlns.com/foaf/0.1/Organization
foaf:Organization rdf:type owl:Class .


###  https://w3id.org/ontouml/2.0.0#AggregationKind
ontouml:AggregationKind rdf:type owl:Class ;
                        owl:equivalentClass [ rdf:type owl:Class ;
                                              owl:oneOf ( ontouml:composite
                                                          ontouml:none
                                                          ontouml:shared
                                                        )
                                            ] ;
                        rdfs:comment "Groups all possible aggregation kinds to which an ontouml:Property can be related."@en ,
                                     "This class is an enumeration of its individuals, which are: ontouml:composite, ontouml:none, and ontouml:shared."@en ;
                        rdfs:isDefinedBy <https://w3id.org/ontouml/2.0.0> ;
                        rdfs:label "Aggregation Kind"@en .


###  https://w3id.org/ontouml/2.0.0#BinaryConnectorView
ontouml:BinaryConnectorView rdf:type owl:Class ;
                            rdfs:subClassOf ontouml:View ;
                            owl:disjointUnionOf ( ontouml:BinaryRelationView
                                                  ontouml:GeneralizationView
                                                ) ;
                            rdfs:comment "An ontouml:View element that represents the single occurrence of a binary connector (e.g., a binary ontouml:Relation, or an ontouml:Generalization) in an ontouml:Diagram."@en ;
                            rdfs:isDefinedBy <https://w3id.org/ontouml/2.0.0> ;
                            rdfs:label "Binary Connector View"@en .


###  https://w3id.org/ontouml/2.0.0#BinaryRelation
ontouml:BinaryRelation rdf:type owl:Class ;
                       rdfs:subClassOf ontouml:Relation ;
                       rdfs:comment """An ontouml:Relation that defines the properties of a set of binary relations of the subject domain.

Examples include \"studies in\", and derivation relations (e.g., between material relations and relators).

A binary relation may either connect two classes, or a relation (as source) and a class (as class) in the case of ontouml:derivation relations connecting descriptive relations to the classes that serve as their truthmakers (as in the relation between the material relation \"studies in\" and the \"Enrollment\" relator)."""@en ;
                       rdfs:isDefinedBy <https://w3id.org/ontouml/2.0.0> ;
                       rdfs:label "Binary Relation"@en ;
                       rdfs:seeAlso <https://doi.org/10.1007/978-3-030-33223-5_4> ,
                                    ontouml:derivation .


###  https://w3id.org/ontouml/2.0.0#BinaryRelationView
ontouml:BinaryRelationView rdf:type owl:Class ;
                           rdfs:subClassOf ontouml:BinaryConnectorView ;
                           rdfs:comment "An ontouml:View element that represents the single occurrence of a ontouml:BinaryRelation in an ontouml:Diagram."@en ;
                           rdfs:isDefinedBy <https://w3id.org/ontouml/2.0.0> ;
                           rdfs:label "Binary Relation View"@en .


###  https://w3id.org/ontouml/2.0.0#Cardinality
ontouml:Cardinality rdf:type owl:Class ;
                    rdfs:comment "Represents the cardinality of an ontouml:Property through its data property ontouml:cardinalityValue."@en ;
                    rdfs:isDefinedBy <https://w3id.org/ontouml/2.0.0> ;
                    rdfs:label "Cardinality"@en .


###  https://w3id.org/ontouml/2.0.0#Class
ontouml:Class rdf:type owl:Class ;
              rdfs:subClassOf ontouml:Classifier ,
                              [ owl:intersectionOf ( [ rdf:type owl:Restriction ;
                                                       owl:onProperty ontouml:stereotype ;
                                                       owl:allValuesFrom ontouml:ClassStereotype
                                                     ]
                                                     [ rdf:type owl:Restriction ;
                                                       owl:onProperty ontouml:stereotype ;
                                                       owl:qualifiedCardinality "1"^^xsd:nonNegativeInteger ;
                                                       owl:onClass ontouml:ClassStereotype
                                                     ]
                                                   ) ;
                                rdf:type owl:Class
                              ] ;
              rdfs:comment """An ontouml:Classifier that defines the properties of a set of \"individualized\" entities (i.e., non-relational) of the subject domain.
              
Examples include \"Person\", \"Enrollment\", and \"Grade\".

The instances of a class may include entities such as objects (e.g., people, organizations, vehicles), reified properties (e.g., leafs' colors, agents' intentions, enrollments), and bare values (e.g., a number or a literal)."""@en ;
              rdfs:isDefinedBy <https://w3id.org/ontouml/2.0.0> ;
              rdfs:label "Class"@en .


###  https://w3id.org/ontouml/2.0.0#ClassStereotype
ontouml:ClassStereotype rdf:type owl:Class ;
                        owl:equivalentClass [ rdf:type owl:Class ;
                                              owl:oneOf ( ontouml:abstract
                                                          ontouml:category
                                                          ontouml:collective
                                                          ontouml:datatype
                                                          ontouml:enumeration
                                                          ontouml:event
                                                          ontouml:historicalRole
                                                          ontouml:historicalRoleMixin
                                                          ontouml:kind
                                                          ontouml:mixin
                                                          ontouml:mode
                                                          ontouml:phase
                                                          ontouml:phaseMixin
                                                          ontouml:quality
                                                          ontouml:quantity
                                                          ontouml:relator
                                                          ontouml:role
                                                          ontouml:roleMixin
                                                          ontouml:situation
                                                          ontouml:subkind
                                                          ontouml:type
                                                        )
                                            ] ;
                        rdfs:subClassOf ontouml:Stereotype ;
                        rdfs:comment "Aggregates all possible instances that can be assigned via an ontouml:stereotype property to an ontouml:Class."@en ,
                                     "This class is an enumeration of its individuals, which are: ontouml:abstract, ontouml:category, ontouml:collective, ontouml:datatype, ontouml:enumeration, ontouml:event, ontouml:historicalRole, ontouml:historicalRoleMixin, ontouml:kind, ontouml:mixin, ontouml:mode, ontouml:phase, ontouml:phaseMixin, ontouml:quality, ontouml:quantity, ontouml:relator, ontouml:role, ontouml:roleMixin, ontouml:situation, ontouml:subkind, and ontouml:type."@en ;
                        rdfs:isDefinedBy <https://w3id.org/ontouml/2.0.0> ;
                        rdfs:label "Class Stereotype"@en .


###  https://w3id.org/ontouml/2.0.0#ClassView
ontouml:ClassView rdf:type owl:Class ;
                  rdfs:subClassOf ontouml:View ;
                  rdfs:comment "An ontouml:View element that represents the single occurrence of an ontouml:Class in an ontouml:Diagram."@en ;
                  rdfs:isDefinedBy <https://w3id.org/ontouml/2.0.0> ;
                  rdfs:label "Class View"@en .


###  https://w3id.org/ontouml/2.0.0#Classifier
ontouml:Classifier rdf:type owl:Class ;
                   rdfs:subClassOf ontouml:DecoratableElement ,
                                   ontouml:PackageableElement ;
                   owl:disjointUnionOf ( ontouml:Class
                                         ontouml:Relation
                                       ) ;
                   rdfs:comment "An ontouml:DecoratableElement (either an ontouml:Class or an ontouml:Relation) that defines properties exhibited by its instances."@en ;
                   rdfs:isDefinedBy <https://w3id.org/ontouml/2.0.0> ;
                   rdfs:label "Classifier"@en ;
                   rdfs:seeAlso ontouml:Class ,
                                ontouml:Relation .


###  https://w3id.org/ontouml/2.0.0#DecoratableElement
ontouml:DecoratableElement rdf:type owl:Class ;
                           rdfs:subClassOf ontouml:ModelElement ;
                           owl:disjointUnionOf ( ontouml:Classifier
                                                 ontouml:Property
                                               ) ;
                           rdfs:comment """An ontouml:ModelElement that can be decorated with a stereotype to identify its ontological properties according to UFO.

Examples include a class decorated with the stereotype \"kind\" identifying it as a type of objects that provides an identity principle to its instances."""@en ;
                           rdfs:isDefinedBy <https://w3id.org/ontouml/2.0.0> ;
                           rdfs:label "Decoratable Element"@en .


###  https://w3id.org/ontouml/2.0.0#Diagram
ontouml:Diagram rdf:type owl:Class ;
                rdfs:subClassOf ontouml:NamedElement ;
                rdfs:comment "An ontouml:NamedElement that contains the visual representation of an OntoUML model or of a portion of it."@en ;
                rdfs:isDefinedBy <https://w3id.org/ontouml/2.0.0> ;
                rdfs:label "Diagram"@en .


###  https://w3id.org/ontouml/2.0.0#Diamond
ontouml:Diamond rdf:type owl:Class ;
                rdfs:subClassOf ontouml:RectangularShape ;
                rdfs:comment "An ontouml:RectangularShape that renders the joining diamond of an ontouml:NaryRelationView."@en ;
                rdfs:isDefinedBy <https://w3id.org/ontouml/2.0.0> ;
                rdfs:label "Rectangular Shape"@en .


###  https://w3id.org/ontouml/2.0.0#Generalization
ontouml:Generalization rdf:type owl:Class ;
                       rdfs:subClassOf ontouml:ModelElement ,
                                       ontouml:PackageableElement ;
                       rdfs:comment """An ontouml:ModelElement that represents the generalization of a specific classifier into a general classifier. When read in the inverse direction, an ontouml:Generalization is referred to as a specialization.

Examples include the generalization of a specific class \"Student\" into a general class \"Person,\" and the generalization of a specific relation \"close friends with\" into a general relation \"friends with\".

A generalization can only connect two classifiers of the same type, i.e., it can either connect two ontouml:Class elements or two ontouml:Relation elements."""@en ;
                       rdfs:isDefinedBy <https://w3id.org/ontouml/2.0.0> ;
                       rdfs:label "Generalization"@en .


###  https://w3id.org/ontouml/2.0.0#GeneralizationSet
ontouml:GeneralizationSet rdf:type owl:Class ;
                          rdfs:subClassOf ontouml:ModelElement ,
                                          ontouml:PackageableElement ;
                          rdfs:comment """An ontouml:ModelElement that represents a group of connected ontouml:Generalization elements. An ontouml:GeneralizationSet can define disjoint and/or complete constraints over the generalizations it groups.

Examples include the incomplete (i.e., non-complete) and overlapping (i.e., non-disjoint) generalization set of \"Person\" into \"Student\" and \"Teacher\", and the disjoint and complete generalization set of \"Person\" into \"Child\" and \"Adult\".

All ontouml:Generalization element in the ontouml:GeneralizationSet must share a common general ontouml:Classifier."""@en ;
                          rdfs:isDefinedBy <https://w3id.org/ontouml/2.0.0> ;
                          rdfs:label "Generalization Set"@en ;
                          rdfs:seeAlso ontouml:GeneralizationSet .


###  https://w3id.org/ontouml/2.0.0#GeneralizationSetView
ontouml:GeneralizationSetView rdf:type owl:Class ;
                              rdfs:subClassOf ontouml:View ;
                              rdfs:comment "An ontouml:View element that represents the single occurrence of an ontouml:Class in an ontouml:Diagram."@en ;
                              rdfs:isDefinedBy <https://w3id.org/ontouml/2.0.0> ;
                              rdfs:label "GeneralizationSetView"@en .


###  https://w3id.org/ontouml/2.0.0#GeneralizationView
ontouml:GeneralizationView rdf:type owl:Class ;
                           rdfs:subClassOf ontouml:BinaryConnectorView ;
                           rdfs:comment "Represents the diagramation (i.e., the visual representation) of an ontouml:Generalization in a given ontouml:Diagram."@en ;
                           rdfs:isDefinedBy <https://w3id.org/ontouml/2.0.0> ;
                           rdfs:label "Generalization View"@en .


###  https://w3id.org/ontouml/2.0.0#Link
ontouml:Link rdf:type owl:Class ;
             rdfs:subClassOf ontouml:ModelElement ,
                             ontouml:PackageableElement ;
             rdfs:comment "An ontouml:ModelElement that connects an ontouml:Note to the ontouml:ModelElement it concerns."@en ;
             rdfs:isDefinedBy <https://w3id.org/ontouml/2.0.0> ;
             rdfs:label "Link"@en .


###  https://w3id.org/ontouml/2.0.0#LinkView
ontouml:LinkView rdf:type owl:Class ;
                 rdfs:subClassOf ontouml:BinaryConnectorView ;
                 rdfs:comment "An ontouml:View element that represents the single occurrence of an ontouml:Link in an ontouml:Diagram."@en ;
                 rdfs:isDefinedBy <https://w3id.org/ontouml/2.0.0> ;
                 rdfs:label "Link View"@en .


###  https://w3id.org/ontouml/2.0.0#Literal
ontouml:Literal rdf:type owl:Class ;
                rdfs:subClassOf ontouml:ModelElement ;
                rdfs:comment "An ontouml:ModelElement that represents a specific value within an enumerated set of values within an ontouml:Class with the ontouml:stereotype ontouml:enumeration. Examples include each letter in an A to F letter grading scale, listed in a class \"Letter Grade\" decorated with the stereotype \"enumeration\"."@en ;
                rdfs:isDefinedBy <https://w3id.org/ontouml/2.0.0> ;
                rdfs:label "Literal"@en ;
                rdfs:seeAlso ontouml:Class ,
                             ontouml:enumeration .


###  https://w3id.org/ontouml/2.0.0#ModelElement
ontouml:ModelElement rdf:type owl:Class ;
                     rdfs:subClassOf ontouml:NamedElement ;
                     owl:disjointUnionOf ( ontouml:DecoratableElement
                                           ontouml:Generalization
                                           ontouml:GeneralizationSet
                                           ontouml:Literal
                                           ontouml:Note
                                           ontouml:Package
                                         ) ;
                     rdfs:comment "An ontouml:NamedElement that represents an element of the language's abstract syntax (e.g., an ontouml:Class, an ontouml:Relation, or an ontouml:Generalization)."@en ;
                     rdfs:isDefinedBy <https://w3id.org/ontouml/2.0.0> ;
                     rdfs:label "Model Element"@en .


###  https://w3id.org/ontouml/2.0.0#NamedElement
ontouml:NamedElement rdf:type owl:Class ;
                     rdfs:subClassOf ontouml:OntoumlElement ;
                     owl:disjointUnionOf ( ontouml:ModelElement
                                           ontouml:Project
                                         ) ;
                     rdfs:comment "An ontouml:ontoumlElement that can be attributed a name and other descriptive information."@en ;
                     rdfs:isDefinedBy <https://w3id.org/ontouml/2.0.0> ;
                     rdfs:label "Named Element"@en .


###  https://w3id.org/ontouml/2.0.0#NaryRelation
ontouml:NaryRelation rdf:type owl:Class ;
                     rdfs:subClassOf ontouml:Relation ;
                     rdfs:comment """An ontouml:Relation that defines the properties of a set of relations of the subject domain that connect more than two members.

Examples include \"studies in\", \"buys product from\" (ternary relation), and derivation relations (e.g., between material relations and relators)."""@en ;
                     rdfs:isDefinedBy <https://w3id.org/ontouml/2.0.0> ;
                     rdfs:label "N-ary Relation"@en .


###  https://w3id.org/ontouml/2.0.0#NaryRelationView
ontouml:NaryRelationView rdf:type owl:Class ;
                         rdfs:subClassOf ontouml:View ;
                         rdfs:comment "An ontouml:View element that represents the single occurrence of an ontouml:NaryRelation in an ontouml:Diagram."@en ;
                         rdfs:isDefinedBy <https://w3id.org/ontouml/2.0.0> ;
                         rdfs:label "N-ary Relation View"@en .


###  https://w3id.org/ontouml/2.0.0#Note
ontouml:Note rdf:type owl:Class ;
             rdfs:subClassOf ontouml:ModelElement ,
                             ontouml:PackageableElement ;
             rdfs:comment "An ontouml:ModelElement that contains an annotation about the ontology or some of its elements. A note can also be used to represent a constraint in both natural or structured language (i.e., first-order logic, or OCL)."@en ;
             rdfs:isDefinedBy <https://w3id.org/ontouml/2.0.0> ;
             rdfs:label "Note"@en .


###  https://w3id.org/ontouml/2.0.0#NoteView
ontouml:NoteView rdf:type owl:Class ;
                 rdfs:subClassOf ontouml:View ;
                 rdfs:comment "An ontouml:View element that represents the single occurrence of an ontouml:Note in an ontouml:Diagram."@en ;
                 rdfs:isDefinedBy <https://w3id.org/ontouml/2.0.0> ;
                 rdfs:label "Note View"@en .


###  https://w3id.org/ontouml/2.0.0#OntologicalNature
ontouml:OntologicalNature rdf:type owl:Class ;
                          owl:equivalentClass [ rdf:type owl:Class ;
                                                owl:oneOf ( ontouml:abstractNature
                                                            ontouml:collectiveNature
                                                            ontouml:eventNature
                                                            ontouml:extrinsicModeNature
                                                            ontouml:functionalComplexNature
                                                            ontouml:intrinsicModeNature
                                                            ontouml:qualityNature
                                                            ontouml:quantityNature
                                                            ontouml:relatorNature
                                                            ontouml:situationNature
                                                            ontouml:typeNature
                                                          )
                                              ] ;
                          rdfs:comment "Collection of individuals that represent fundamental conceptual modeling issues according to the Unified Foundational Ontology (UFO) theory."@en ,
                                       "This class is an enumeration of its individuals, which are: ontouml:abstractNature, ontouml:collectiveNature, ontouml:eventNature, ontouml:extrinsicModeNature, ontouml:functionalComplexNature, ontouml:intrinsicModeNature, ontouml:qualityNature, ontouml:quantityNature, ontouml:relatorNature, ontouml:situationNature, and ontouml:typeNature."@en ;
                          rdfs:isDefinedBy <https://w3id.org/ontouml/2.0.0> ;
                          rdfs:label "Ontological Nature"@en ;
                          rdfs:seeAlso <https://doi.org/10.3233/AO-150157> .


###  https://w3id.org/ontouml/2.0.0#OntoumlElement
ontouml:OntoumlElement rdf:type owl:Class ;
                       rdfs:comment "An identified element of an OntoUML ontology according to the OntoUML Metamodel, which includes projects, model elements, diagrams, views, and shapes."@en ;
                       rdfs:isDefinedBy <https://w3id.org/ontouml/2.0.0> ;
                       rdfs:label "OntoUML Element"@en .


###  https://w3id.org/ontouml/2.0.0#Package
ontouml:Package rdf:type owl:Class ;
                rdfs:subClassOf ontouml:ModelElement ;
                rdfs:comment """An ontouml:ModelElement that groups other model elements referred to as \"packageable elements.\" Package elements are used to perform the modularization of an ontology.
                
While the OntoUML Metamodel does not require package elements to follow a tree structure (i.e., it allows overlapping packages), ontologies that require UML representations should adhere to this constraint for compatibility."""@en ;
                rdfs:isDefinedBy <https://w3id.org/ontouml/2.0.0> ;
                rdfs:label "Package"@en .


###  https://w3id.org/ontouml/2.0.0#PackageView
ontouml:PackageView rdf:type owl:Class ;
                    rdfs:subClassOf ontouml:View ;
                    rdfs:comment "An ontouml:View element that represents the single occurrence of an ontouml:Package in an ontouml:Diagram."@en ;
                    rdfs:isDefinedBy <https://w3id.org/ontouml/2.0.0> ;
                    rdfs:label "Package View"@en .


###  https://w3id.org/ontouml/2.0.0#PackageableElement
ontouml:PackageableElement rdf:type owl:Class ;
                           rdfs:subClassOf ontouml:ModelElement ;
                           rdfs:comment "An ontouml:ModelElement that can be grouped into an ontouml:Package."@en ;
                           rdfs:isDefinedBy <https://w3id.org/ontouml/2.0.0> ;
                           rdfs:label "Packageable Element"@en .


###  https://w3id.org/ontouml/2.0.0#Path
ontouml:Path rdf:type owl:Class ;
             rdfs:subClassOf ontouml:Shape ;
             rdfs:comment "An ontouml:Shape defined by a list of ontouml:Point values connecting two other ontouml:Shape elements."@en ;
             rdfs:isDefinedBy <https://w3id.org/ontouml/2.0.0> ;
             rdfs:label "Path"@en .


###  https://w3id.org/ontouml/2.0.0#Point
ontouml:Point rdf:type owl:Class ;
              rdfs:comment "Contains the ontouml:xCoordinate value and ontouml:yCoordinate value. These values represent the top left position of an ontouml:RectangularShape, to which the ontouml:Point is related vian ontouml:topLeftPosition property."@en ;
              rdfs:isDefinedBy <https://w3id.org/ontouml/2.0.0> ;
              rdfs:label "Point"@en .


###  https://w3id.org/ontouml/2.0.0#Project
ontouml:Project rdf:type owl:Class ;
                rdfs:subClassOf ontouml:NamedElement ;
                rdfs:comment "An ontouml:NamedElement that serves as the container of an entire OntoUML ontology, including the elements of both the abstract syntax (i.e., model elements) and the concrete syntax (i.e., diagrams, view, and shapes)."@en ;
                rdfs:isDefinedBy <https://w3id.org/ontouml/2.0.0> ;
                rdfs:label "Project"@en .


###  https://w3id.org/ontouml/2.0.0#Property
ontouml:Property rdf:type owl:Class ;
                 rdfs:subClassOf ontouml:DecoratableElement ,
                                 [ owl:intersectionOf ( [ rdf:type owl:Restriction ;
                                                          owl:onProperty ontouml:stereotype ;
                                                          owl:allValuesFrom ontouml:PropertyStereotype
                                                        ]
                                                        [ rdf:type owl:Restriction ;
                                                          owl:onProperty ontouml:stereotype ;
                                                          owl:maxQualifiedCardinality "1"^^xsd:nonNegativeInteger ;
                                                          owl:onClass ontouml:PropertyStereotype
                                                        ]
                                                      ) ;
                                   rdf:type owl:Class
                                 ] ;
                 rdfs:comment """An ontouml:DecoratableElement that represents an attribute of an ontouml:Class, or one end of an ontouml:Relation.

Examples include the attribute \"name\" of the class \"Person\", and the ends of the binary relation \"studies in\" connected to the classes \"Student\" and \"University.\"

Instances of class and relation elements bear values for the properties these classifiers contain, according to the constraints specified within each property. For example, the value assigned to a property in an instance must be itself an instance of the classifier in property type."""@en ;
                 rdfs:isDefinedBy <https://w3id.org/ontouml/2.0.0> ;
                 rdfs:label "Property"@en .


###  https://w3id.org/ontouml/2.0.0#PropertyStereotype
ontouml:PropertyStereotype rdf:type owl:Class ;
                           owl:equivalentClass [ rdf:type owl:Class ;
                                                 owl:oneOf ( ontouml:begin
                                                             ontouml:end
                                                           )
                                               ] ;
                           rdfs:subClassOf ontouml:Stereotype ;
                           rdfs:comment "Aggregates all possible instances that can be assigned via an ontouml:stereotype property to an ontouml:Property."@en ,
                                        "This class is an enumeration of its individuals, which are: ontouml:begin, and ontouml:end."@en ;
                           rdfs:isDefinedBy <https://w3id.org/ontouml/2.0.0> ;
                           rdfs:label "Property Stereotype"@en .


###  https://w3id.org/ontouml/2.0.0#Rectangle
ontouml:Rectangle rdf:type owl:Class ;
                  rdfs:subClassOf ontouml:RectangularShape ;
                  rdfs:comment "An ontouml:RectangularShape that renders the shape of an ontouml:ClassView or an ontouml:PackageView."@en ;
                  rdfs:isDefinedBy <https://w3id.org/ontouml/2.0.0> ;
                  rdfs:label "Rectangle"@en .


###  https://w3id.org/ontouml/2.0.0#RectangularShape
ontouml:RectangularShape rdf:type owl:Class ;
                         rdfs:subClassOf ontouml:Shape ;
                         owl:disjointUnionOf ( ontouml:Diamond
                                               ontouml:Rectangle
                                               ontouml:Text
                                             ) ;
                         rdfs:comment "An ontouml:Shape defined by an ontouml:topLeftPosition, an ontouml:height, and an ontouml:width."@en ;
                         rdfs:isDefinedBy <https://w3id.org/ontouml/2.0.0> ;
                         rdfs:label "Rectangular Shape"@en .


###  https://w3id.org/ontouml/2.0.0#Relation
ontouml:Relation rdf:type owl:Class ;
                 rdfs:subClassOf ontouml:Classifier ,
                                 [ owl:intersectionOf ( [ rdf:type owl:Restriction ;
                                                          owl:onProperty ontouml:stereotype ;
                                                          owl:allValuesFrom ontouml:RelationStereotype
                                                        ]
                                                        [ rdf:type owl:Restriction ;
                                                          owl:onProperty ontouml:stereotype ;
                                                          owl:maxQualifiedCardinality "1"^^xsd:nonNegativeInteger ;
                                                          owl:onClass ontouml:RelationStereotype
                                                        ]
                                                      ) ;
                                   rdf:type owl:Class
                                 ] ;
                 rdfs:comment """An ontouml:Classifier that defines the properties of a set of relations of the subject domain.

Examples include \"studies in\", \"buys product from\" (ternary relation), and derivation relations (e.g., between material relations and relators)."""@en ;
                 rdfs:isDefinedBy <https://w3id.org/ontouml/2.0.0> ;
                 rdfs:label "Relation"@en .


###  https://w3id.org/ontouml/2.0.0#RelationStereotype
ontouml:RelationStereotype rdf:type owl:Class ;
                           owl:equivalentClass [ rdf:type owl:Class ;
                                                 owl:oneOf ( ontouml:bringsAbout
                                                             ontouml:characterization
                                                             ontouml:comparative
                                                             ontouml:componentOf
                                                             ontouml:creation
                                                             ontouml:derivation
                                                             ontouml:externalDependence
                                                             ontouml:historicalDependence
                                                             ontouml:instantiation
                                                             ontouml:manifestation
                                                             ontouml:material
                                                             ontouml:mediation
                                                             ontouml:memberOf
                                                             ontouml:participation
                                                             ontouml:participational
                                                             ontouml:subCollectionOf
                                                             ontouml:subQuantityOf
                                                             ontouml:termination
                                                             ontouml:triggers
                                                           )
                                               ] ;
                           rdfs:subClassOf ontouml:Stereotype ;
                           rdfs:comment "Aggregates all possible instances that can be assigned via an ontouml:stereotype property to an ontouml:Relation."@en ,
                                        "This class is an enumeration of its individuals, which are: ontouml:bringsAbout, ontouml:characterization, ontouml:comparative, ontouml:componentOf, ontouml:creation, ontouml:derivation, ontouml:externalDependence, ontouml:historicalDependence, ontouml:instantiation, ontouml:manifestation, ontouml:material, ontouml:mediation, ontouml:memberOf, ontouml:participation, ontouml:participational, ontouml:subCollectionOf, ontouml:subQuantityOf, ontouml:termination, and ontouml:triggers."@en ;
                           rdfs:isDefinedBy <https://w3id.org/ontouml/2.0.0> ;
                           rdfs:label "Relation Stereotype"@en .


###  https://w3id.org/ontouml/2.0.0#SemanticArtefact
ontouml:SemanticArtefact rdf:type owl:Class .


###  https://w3id.org/ontouml/2.0.0#SemanticArtefactTask
ontouml:SemanticArtefactTask rdf:type owl:Class .


###  https://w3id.org/ontouml/2.0.0#Shape
ontouml:Shape rdf:type owl:Class ;
              rdfs:subClassOf ontouml:OntoumlElement ;
              owl:disjointUnionOf ( ontouml:Path
                                    ontouml:RectangularShape
                                  ) ;
              rdfs:comment "An ontouml:OntoumlElement that identifies how to render an ontouml:View (or a portion of one) in an ontouml:Diagram."@en ;
              rdfs:isDefinedBy <https://w3id.org/ontouml/2.0.0> ;
              rdfs:label "Shape"@en .


###  https://w3id.org/ontouml/2.0.0#Stereotype
ontouml:Stereotype rdf:type owl:Class ;
                   owl:disjointUnionOf ( ontouml:ClassStereotype
                                         ontouml:PropertyStereotype
                                         ontouml:RelationStereotype
                                       ) ;
                   rdfs:comment "Indicates meta-properties of classes, properties, or relations."@en ;
                   rdfs:isDefinedBy <https://w3id.org/ontouml/2.0.0> ;
                   rdfs:label "Stereotype"@en .


###  https://w3id.org/ontouml/2.0.0#Text
ontouml:Text rdf:type owl:Class ;
             rdfs:subClassOf ontouml:RectangularShape ;
             rdfs:comment "An ontouml:RectangularShape that renders the shape of an ontouml:GeneralizationSetView or an ontouml:NoteView."@en ;
             rdfs:isDefinedBy <https://w3id.org/ontouml/2.0.0> ;
             rdfs:label "Text"@en .


###  https://w3id.org/ontouml/2.0.0#View
ontouml:View rdf:type owl:Class ;
             rdfs:subClassOf ontouml:OntoumlElement ;
             rdfs:comment """An ontouml:OntoumlElement that represents a single ontouml:ModelElement in a ontouml:Diagram.

A view element connects a model element to the shapes in a diagram necessary to represent a single occurrence of it. For example, an n-ary relation view connects a single relation element to one diamond and a set of paths that represent a single occurrence of it in a diagram. Multiple views can represent multiple occurrences of an element in the same diagram.
      
A view element is responsible for what portions of a model element are present in a single diagram representation (e.g., whether the cardinality of a property is shown), unlike a shape, which is responsible aspects of the actual drawing (e.g., how to render a portion of a view, in which position, and with which dimensions)."""@en ;
             rdfs:isDefinedBy <https://w3id.org/ontouml/2.0.0> ;
             rdfs:label "Element View"@en ;
             rdfs:seeAlso ontouml:Shape .


#################################################################
#    Individuals
#################################################################

###  https://creativecommons.org/licenses/by-sa/4.0
<https://creativecommons.org/licenses/by-sa/4.0> rdf:type owl:NamedIndividual .


###  https://w3id.org/ontouml
<https://w3id.org/ontouml> rdf:type owl:NamedIndividual ,
                                    dct:Standard .


###  https://w3id.org/ontouml/vocabulary
<https://w3id.org/ontouml/vocabulary> rdf:type owl:NamedIndividual .


###  https://w3id.org/ontouml/2.0.0
<https://w3id.org/ontouml/2.0.0> rdf:type owl:NamedIndividual .


###  https://w3id.org/ontouml/2.0.0#abstract
ontouml:abstract rdf:type owl:NamedIndividual ,
                          ontouml:ClassStereotype ;
                 rdfs:comment "An individual of the ontouml:ClassStereotype used to assign the corresponding stereotype to a given ontouml:Class."@en ;
                 rdfs:isDefinedBy <https://w3id.org/ontouml/2.0.0> ;
                 rdfs:label "abstract"@en .


###  https://w3id.org/ontouml/2.0.0#abstractNature
ontouml:abstractNature rdf:type owl:NamedIndividual ,
                                ontouml:OntologicalNature ;
                       rdfs:comment "Indicates that the restricted type includes abstract individuals among its instances."@en ;
                       rdfs:isDefinedBy <https://w3id.org/ontouml/2.0.0> ;
                       rdfs:label "abstract nature"@en .


###  https://w3id.org/ontouml/2.0.0#begin
ontouml:begin rdf:type owl:NamedIndividual ,
                       ontouml:PropertyStereotype ;
              rdfs:comment "An individual of the ontouml:PropertyStereotype used to assign the corresponding stereotype to a given ontouml:Property."@en ;
              rdfs:isDefinedBy <https://w3id.org/ontouml/2.0.0> ;
              rdfs:label "begin"@en ;
              rdfs:seeAlso <https://doi.org/10.1007/978-3-030-33223-5_39> .


###  https://w3id.org/ontouml/2.0.0#bringsAbout
ontouml:bringsAbout rdf:type owl:NamedIndividual ,
                             ontouml:RelationStereotype ;
                    rdfs:comment "An individual of the ontouml:RelationStereotype used to assign the corresponding stereotype to a given ontouml:Relation."@en ;
                    rdfs:isDefinedBy <https://w3id.org/ontouml/2.0.0> ;
                    rdfs:label "brings about"@en ;
                    rdfs:seeAlso <https://doi.org/10.1007/978-3-030-33223-5_39> .


###  https://w3id.org/ontouml/2.0.0#category
ontouml:category rdf:type owl:NamedIndividual ,
                          ontouml:ClassStereotype ;
                 rdfs:comment "A rigid mixin that does not require a dependency to be specified. It is used to aggregate essential properties of individuals following different identity principles."@en ;
                 rdfs:isDefinedBy <https://w3id.org/ontouml/2.0.0> ;
                 rdfs:label "category"@en ;
                 rdfs:seeAlso "https://ontouml.readthedocs.io/en/latest/classes/nonsortals/category/index.html"^^xsd:anyURI .


###  https://w3id.org/ontouml/2.0.0#characterization
ontouml:characterization rdf:type owl:NamedIndividual ,
                                  ontouml:RelationStereotype ;
                         rdfs:comment "An ontouml:RelationStereotype attributed to a relation between a bearer type and its feature."@en ;
                         rdfs:isDefinedBy <https://w3id.org/ontouml/2.0.0> ;
                         rdfs:label "characterization"@en ;
                         rdfs:seeAlso <https://doi.org/10.1007/978-3-030-33223-5_4> ,
                                      "https://ontouml.readthedocs.io/en/latest/relationships/characterization/index.html"^^xsd:anyURI .


###  https://w3id.org/ontouml/2.0.0#collective
ontouml:collective rdf:type owl:NamedIndividual ,
                            ontouml:ClassStereotype ;
                   rdfs:comment "An ontouml:ClassStereotype used to represent rigid concepts that provide an identity principle for their instances."@en ;
                   rdfs:isDefinedBy <https://w3id.org/ontouml/2.0.0> ;
                   rdfs:label "collective"@en ;
                   rdfs:seeAlso "https://ontouml.readthedocs.io/en/latest/classes/sortals/collective/index.html"^^xsd:anyURI .


###  https://w3id.org/ontouml/2.0.0#collectiveNature
ontouml:collectiveNature rdf:type owl:NamedIndividual ,
                                  ontouml:OntologicalNature ;
                         rdfs:comment "Indicates that the restricted type includes collective individuals among its instances."@en ;
                         rdfs:isDefinedBy <https://w3id.org/ontouml/2.0.0> ;
                         rdfs:label "collective nature"@en .


###  https://w3id.org/ontouml/2.0.0#comparative
ontouml:comparative rdf:type owl:NamedIndividual ,
                             ontouml:RelationStereotype ;
                    rdfs:comment "The stereotype for comparative relations (e.g., heavier-than). Decorates relations that always hold between any two individuals bearing the same relevant quality."@en ;
                    rdfs:isDefinedBy <https://w3id.org/ontouml/2.0.0> ;
                    rdfs:label "comparative"@en ;
                    rdfs:seeAlso <https://doi.org/10.1007/978-3-030-33223-5_4> .


###  https://w3id.org/ontouml/2.0.0#componentOf
ontouml:componentOf rdf:type owl:NamedIndividual ,
                             ontouml:RelationStereotype ;
                    rdfs:comment "A parthood relation between two complexes."@en ;
                    rdfs:isDefinedBy <https://w3id.org/ontouml/2.0.0> ;
                    rdfs:label "component of"@en ;
                    rdfs:seeAlso "https://ontouml.readthedocs.io/en/latest/relationships/aggregations/componentOf/index.html"^^xsd:anyURI .


###  https://w3id.org/ontouml/2.0.0#composite
ontouml:composite rdf:type owl:NamedIndividual ,
                           ontouml:AggregationKind ;
                  rdfs:comment "The value denoting that an ontouml:Property represents a composite aggregation, i.e., a strong form of aggregation."@en ;
                  rdfs:isDefinedBy <https://w3id.org/ontouml/2.0.0> ;
                  rdfs:label "composite"@en .


###  https://w3id.org/ontouml/2.0.0#creation
ontouml:creation rdf:type owl:NamedIndividual ,
                          ontouml:RelationStereotype ;
                 rdfs:comment "An individual of the ontouml:RelationStereotype used to assign the corresponding stereotype to a given ontouml:Relation."@en ;
                 rdfs:isDefinedBy <https://w3id.org/ontouml/2.0.0> ;
                 rdfs:label "creation"@en ;
                 rdfs:seeAlso <https://doi.org/10.1007/978-3-030-33223-5_39> .


###  https://w3id.org/ontouml/2.0.0#datatype
ontouml:datatype rdf:type owl:NamedIndividual ,
                          ontouml:ClassStereotype ;
                 rdfs:comment "An individual of the ontouml:ClassStereotype used to assign the corresponding stereotype to a given ontouml:Class."@en ;
                 rdfs:isDefinedBy <https://w3id.org/ontouml/2.0.0> ;
                 rdfs:label "datatype"@en .


###  https://w3id.org/ontouml/2.0.0#derivation
ontouml:derivation rdf:type owl:NamedIndividual ,
                            ontouml:RelationStereotype ;
                   rdfs:comment "An individual of the ontouml:RelationStereotype used to assign the corresponding stereotype to a given ontouml:Relation."@en ;
                   rdfs:isDefinedBy <https://w3id.org/ontouml/2.0.0> ;
                   rdfs:label "derivation"@en .


###  https://w3id.org/ontouml/2.0.0#end
ontouml:end rdf:type owl:NamedIndividual ,
                     ontouml:PropertyStereotype ;
            rdfs:comment "An individual of the ontouml:PropertyStereotype used to assign the corresponding stereotype to a given ontouml:Property."@en ;
            rdfs:isDefinedBy <https://w3id.org/ontouml/2.0.0> ;
            rdfs:label "end"@en ;
            rdfs:seeAlso <https://doi.org/10.1007/978-3-030-33223-5_39> .


###  https://w3id.org/ontouml/2.0.0#enumeration
ontouml:enumeration rdf:type owl:NamedIndividual ,
                             ontouml:ClassStereotype ;
                    rdfs:comment "Represents the enumeration stereotype, having values represented using ontouml:Literal instances."@en ;
                    rdfs:isDefinedBy <https://w3id.org/ontouml/2.0.0> ;
                    rdfs:label "enumeration"@en .


###  https://w3id.org/ontouml/2.0.0#event
ontouml:event rdf:type owl:NamedIndividual ,
                       ontouml:ClassStereotype ;
              rdfs:comment "An individual of the ontouml:ClassStereotype used to assign the corresponding stereotype to a given ontouml:Class."@en ,
                           "Things that happen to or are performed by endurants (Casati and Varzi, 2015)."@en ;
              rdfs:isDefinedBy <https://w3id.org/ontouml/2.0.0> ;
              rdfs:label "event"@en ;
              rdfs:seeAlso <https://doi.org/10.1007/978-3-030-33223-5_39> .


###  https://w3id.org/ontouml/2.0.0#eventNature
ontouml:eventNature rdf:type owl:NamedIndividual ,
                             ontouml:OntologicalNature ;
                    rdfs:comment "Indicates that the restricted type includes event individuals among its instances."@en ;
                    rdfs:isDefinedBy <https://w3id.org/ontouml/2.0.0> ;
                    rdfs:label "event nature"@en .


###  https://w3id.org/ontouml/2.0.0#externalDependence
ontouml:externalDependence rdf:type owl:NamedIndividual ,
                                    ontouml:RelationStereotype ;
                           rdfs:comment "Identifies an endurant on which the extrinsicMode depends."@en ;
                           rdfs:isDefinedBy <https://w3id.org/ontouml/2.0.0> ;
                           rdfs:label "external dependence"@en ;
                           rdfs:seeAlso <https://doi.org/10.1007/978-3-030-33223-5_4> ,
                                        "https://nemo-ufes.github.io/gufo/#externallyDependsOn"^^xsd:anyURI .


###  https://w3id.org/ontouml/2.0.0#extrinsicModeNature
ontouml:extrinsicModeNature rdf:type owl:NamedIndividual ,
                                     ontouml:OntologicalNature ;
                            rdfs:comment "Identifies what inheres in a concrete individual and depends on others for its existence."@en ;
                            rdfs:isDefinedBy <https://w3id.org/ontouml/2.0.0> ;
                            rdfs:label "extrinsic mode nature"@en .


###  https://w3id.org/ontouml/2.0.0#functionalComplexNature
ontouml:functionalComplexNature rdf:type owl:NamedIndividual ,
                                         ontouml:OntologicalNature ;
                                rdfs:comment "Identifies the nature of a complex object whose parts (components) play different roles in its composition."@en ;
                                rdfs:isDefinedBy <https://w3id.org/ontouml/2.0.0> ;
                                rdfs:label "functional-complex nature"@en .


###  https://w3id.org/ontouml/2.0.0#historicalDependence
ontouml:historicalDependence rdf:type owl:NamedIndividual ,
                                      ontouml:RelationStereotype ;
                             rdfs:comment "Identifies a concrete individual on which another concrete individual depends historically."@en ;
                             rdfs:isDefinedBy <https://w3id.org/ontouml/2.0.0> ;
                             rdfs:label "historical dependence"@en ;
                             rdfs:seeAlso <https://doi.org/10.1007/978-3-030-33223-5_39> .


###  https://w3id.org/ontouml/2.0.0#historicalRole
ontouml:historicalRole rdf:type owl:NamedIndividual ,
                                ontouml:ClassStereotype ;
                       rdfs:comment "Denotes the role of an endurant in virtue of having participated in an event of a particular type."@en ;
                       rdfs:isDefinedBy <https://w3id.org/ontouml/2.0.0> ;
                       rdfs:label "historical role"@en ;
                       rdfs:seeAlso <https://doi.org/10.1007/978-3-030-33223-5_39> .


###  https://w3id.org/ontouml/2.0.0#historicalRoleMixin
ontouml:historicalRoleMixin rdf:type owl:NamedIndividual ,
                                     ontouml:ClassStereotype ;
                            rdfs:comment "Denotes the equivalent of historicalRole for types that aggregate instances with different identity principles."@en ;
                            rdfs:isDefinedBy <https://w3id.org/ontouml/2.0.0> ;
                            rdfs:label "historical role mixin"@en ;
                            rdfs:seeAlso <https://doi.org/10.1007/978-3-030-33223-5_39> .


###  https://w3id.org/ontouml/2.0.0#instantiation
ontouml:instantiation rdf:type owl:NamedIndividual ,
                               ontouml:RelationStereotype ;
                      rdfs:comment "An individual of the ontouml:RelationStereotype used to assign the corresponding stereotype to a given ontouml:Relation."@en ;
                      rdfs:isDefinedBy <https://w3id.org/ontouml/2.0.0> ;
                      rdfs:label "instantiation"@en .


###  https://w3id.org/ontouml/2.0.0#intrinsicModeNature
ontouml:intrinsicModeNature rdf:type owl:NamedIndividual ,
                                     ontouml:OntologicalNature ;
                            rdfs:comment "Indicates that the restricted type includes intrinsic mode individuals among its instances."@en ;
                            rdfs:isDefinedBy <https://w3id.org/ontouml/2.0.0> ;
                            rdfs:label "intrinsic mode nature"@en .


###  https://w3id.org/ontouml/2.0.0#kind
ontouml:kind rdf:type owl:NamedIndividual ,
                      ontouml:ClassStereotype ;
             rdfs:comment "Used to represent rigid concepts that provide an identity principle for their instances and do not require a relational dependency."@en ;
             rdfs:isDefinedBy <https://w3id.org/ontouml/2.0.0> ;
             rdfs:label "kind"@en ;
             rdfs:seeAlso "https://ontouml.readthedocs.io/en/latest/classes/sortals/kind/index.html"^^xsd:anyURI .


###  https://w3id.org/ontouml/2.0.0#manifestation
ontouml:manifestation rdf:type owl:NamedIndividual ,
                               ontouml:RelationStereotype ;
                      rdfs:comment "An individual of the ontouml:RelationStereotype used to assign the corresponding stereotype to a given ontouml:Relation."@en ;
                      rdfs:isDefinedBy <https://w3id.org/ontouml/2.0.0> ;
                      rdfs:label "manifestation"@en .


###  https://w3id.org/ontouml/2.0.0#material
ontouml:material rdf:type owl:NamedIndividual ,
                          ontouml:RelationStereotype ;
                 rdfs:comment "Identifies relations that have material structure on their own and include examples such as employments, kisses, enrollments, flight, connections and commitments."@en ;
                 rdfs:isDefinedBy <https://w3id.org/ontouml/2.0.0> ;
                 rdfs:label "material"@en ;
                 rdfs:seeAlso <https://doi.org/10.1007/978-3-030-33223-5_4> ,
                              "https://ontouml.readthedocs.io/en/latest/relationships/material/index.html"^^xsd:anyURI .


###  https://w3id.org/ontouml/2.0.0#mediation
ontouml:mediation rdf:type owl:NamedIndividual ,
                           ontouml:RelationStereotype ;
                  rdfs:comment "A type of existential dependence relation (a form of nonfunctional inherence). It can be derived from the relation between the relata and the qua individuals that compose the relator and that inhere in the relata."@en ;
                  rdfs:isDefinedBy <https://w3id.org/ontouml/2.0.0> ;
                  rdfs:label "mediation"@en ;
                  rdfs:seeAlso <https://doi.org/10.1007/978-3-030-33223-5_4> ,
                               "https://ontouml.readthedocs.io/en/latest/relationships/mediation/index.html"^^xsd:anyURI .


###  https://w3id.org/ontouml/2.0.0#memberOf
ontouml:memberOf rdf:type owl:NamedIndividual ,
                          ontouml:RelationStereotype ;
                 rdfs:comment "A parthood relation between a functional complex or a Collective (as a part) and a Collective (as a whole)."@en ;
                 rdfs:isDefinedBy <https://w3id.org/ontouml/2.0.0> ;
                 rdfs:label "member of"@en ;
                 rdfs:seeAlso "https://ontouml.readthedocs.io/en/latest/relationships/aggregations/memberOf/index.html"^^xsd:anyURI .


###  https://w3id.org/ontouml/2.0.0#mixin
ontouml:mixin rdf:type owl:NamedIndividual ,
                       ontouml:ClassStereotype ;
              rdfs:comment "Represents a semi-rigid type, i.e., it behaves as a rigid type for some individuals and as an anti-rigid one for others."@en ;
              rdfs:isDefinedBy <https://w3id.org/ontouml/2.0.0> ;
              rdfs:label "mixin"@en ;
              rdfs:seeAlso "https://ontouml.readthedocs.io/en/latest/classes/nonsortals/mixin/index.html"^^xsd:anyURI .


###  https://w3id.org/ontouml/2.0.0#mode
ontouml:mode rdf:type owl:NamedIndividual ,
                      ontouml:ClassStereotype ;
             rdfs:comment "A particular type of intrinsic property that has no structured value."@en ;
             rdfs:isDefinedBy <https://w3id.org/ontouml/2.0.0> ;
             rdfs:label "mode"@en ;
             rdfs:seeAlso "https://ontouml.readthedocs.io/en/latest/classes/aspects/mode/index.html"^^xsd:anyURI .


###  https://w3id.org/ontouml/2.0.0#none
ontouml:none rdf:type owl:NamedIndividual ,
                      ontouml:AggregationKind ;
             rdfs:comment "Denotes that an ontouml:Property is neither ontouml:shared nor ontouml:composite, but just an aggregation."@en ;
             rdfs:isDefinedBy <https://w3id.org/ontouml/2.0.0> ;
             rdfs:label "none"@en .


###  https://w3id.org/ontouml/2.0.0#participation
ontouml:participation rdf:type owl:NamedIndividual ,
                               ontouml:RelationStereotype ;
                      rdfs:comment "A relation for representing when an event depends on a single object."@en ;
                      rdfs:isDefinedBy <https://w3id.org/ontouml/2.0.0> ;
                      rdfs:label "participation"@en ;
                      rdfs:seeAlso <https://doi.org/10.1007/978-3-030-33223-5_39> .


###  https://w3id.org/ontouml/2.0.0#participational
ontouml:participational rdf:type owl:NamedIndividual ,
                                 ontouml:RelationStereotype ;
                        rdfs:comment "Denotes a kind of event decomposition."@en ;
                        rdfs:isDefinedBy <https://w3id.org/ontouml/2.0.0> ;
                        rdfs:label "participational"@en ;
                        rdfs:seeAlso <https://doi.org/10.1007/978-3-030-33223-5_39> .


###  https://w3id.org/ontouml/2.0.0#phase
ontouml:phase rdf:type owl:NamedIndividual ,
                       ontouml:ClassStereotype ;
              rdfs:comment "Used to represent anti-rigid subtypes of identity providers (Kind, Collective, Quantity, Relator, Mode, and Quantity) that are instantiated by changes in intrinsic properties (e.g., the age of a person, the color of an object, the condition of a car).Phases always come in partitions."@en ;
              rdfs:isDefinedBy <https://w3id.org/ontouml/2.0.0> ;
              rdfs:label "phase"@en ;
              rdfs:seeAlso "https://ontouml.readthedocs.io/en/latest/classes/sortals/phase/index.html"^^xsd:anyURI .


###  https://w3id.org/ontouml/2.0.0#phaseMixin
ontouml:phaseMixin rdf:type owl:NamedIndividual ,
                            ontouml:ClassStereotype ;
                   rdfs:comment "The equivalent of Phase for types that aggregate instances with different identity principles. A class stereotyped as PhaseMixin is also an anti-rigid type. PhaseMixin is similar semantically to RoleMixin with the difference in relational dependency."@en ;
                   rdfs:isDefinedBy <https://w3id.org/ontouml/2.0.0> ;
                   rdfs:label "phase mixin"@en ;
                   rdfs:seeAlso "https://ontouml.readthedocs.io/en/latest/classes/nonsortals/phasemixin/index.html"^^xsd:anyURI .


###  https://w3id.org/ontouml/2.0.0#quality
ontouml:quality rdf:type owl:NamedIndividual ,
                         ontouml:ClassStereotype ;
                rdfs:comment "A Quality is a particular type of intrinsic property that has a structured value. Qualities are things that existentially depend on the things they characterize, called their bearers."@en ;
                rdfs:isDefinedBy <https://w3id.org/ontouml/2.0.0> ;
                rdfs:label "quality"@en ;
                rdfs:seeAlso "https://ontouml.readthedocs.io/en/latest/classes/aspects/quality/index.html"^^xsd:anyURI .


###  https://w3id.org/ontouml/2.0.0#qualityNature
ontouml:qualityNature rdf:type owl:NamedIndividual ,
                               ontouml:OntologicalNature ;
                      rdfs:comment "Indicates that the restricted type includes quality individuals among its instances."@en ;
                      rdfs:isDefinedBy <https://w3id.org/ontouml/2.0.0> ;
                      rdfs:label "quality nature"@en .


###  https://w3id.org/ontouml/2.0.0#quantity
ontouml:quantity rdf:type owl:NamedIndividual ,
                          ontouml:ClassStereotype ;
                 rdfs:comment "Construct used to represent rigid concepts that provide an identity principle for their instances."@en ;
                 rdfs:isDefinedBy <https://w3id.org/ontouml/2.0.0> ;
                 rdfs:label "quantity"@en ;
                 rdfs:seeAlso "https://ontouml.readthedocs.io/en/latest/classes/sortals/quantity/index.html"^^xsd:anyURI .


###  https://w3id.org/ontouml/2.0.0#quantityNature
ontouml:quantityNature rdf:type owl:NamedIndividual ,
                                ontouml:OntologicalNature ;
                       rdfs:comment "Indicates that the restricted type includes quantity individuals among its instances."@en ;
                       rdfs:isDefinedBy <https://w3id.org/ontouml/2.0.0> ;
                       rdfs:label "quantity nature"@en .


###  https://w3id.org/ontouml/2.0.0#relator
ontouml:relator rdf:type owl:NamedIndividual ,
                         ontouml:ClassStereotype ;
                rdfs:comment "A construct used to represent truth-makers of material relations, i.e., the things that must exist for two or more individuals to be connected by material relations."@en ;
                rdfs:isDefinedBy <https://w3id.org/ontouml/2.0.0> ;
                rdfs:label "relator"@en ;
                rdfs:seeAlso "https://ontouml.readthedocs.io/en/latest/classes/sortals/relator/index.html"^^xsd:anyURI .


###  https://w3id.org/ontouml/2.0.0#relatorNature
ontouml:relatorNature rdf:type owl:NamedIndividual ,
                               ontouml:OntologicalNature ;
                      rdfs:comment "Indicates that the restricted type includes relator individuals among its instances."@en ;
                      rdfs:isDefinedBy <https://w3id.org/ontouml/2.0.0> ;
                      rdfs:label "relator nature"@en .


###  https://w3id.org/ontouml/2.0.0#role
ontouml:role rdf:type owl:NamedIndividual ,
                      ontouml:ClassStereotype ;
             rdfs:comment "Used to represent anti-rigid specializations of identity providers (Kind, Collective, Quantity, Relator, Mode, and Quantity) that are instantiated in relational contexts."@en ;
             rdfs:isDefinedBy <https://w3id.org/ontouml/2.0.0> ;
             rdfs:label "role"@en ;
             rdfs:seeAlso "https://ontouml.readthedocs.io/en/latest/classes/sortals/role/index.html"^^xsd:anyURI .


###  https://w3id.org/ontouml/2.0.0#roleMixin
ontouml:roleMixin rdf:type owl:NamedIndividual ,
                           ontouml:ClassStereotype ;
                  rdfs:comment "The equivalent of Role for types that aggregate instances with different identity principles."@en ;
                  rdfs:isDefinedBy <https://w3id.org/ontouml/2.0.0> ;
                  rdfs:label "role mixin"@en ;
                  rdfs:seeAlso "https://ontouml.readthedocs.io/en/latest/classes/nonsortals/rolemixin/index.html"^^xsd:anyURI .


###  https://w3id.org/ontouml/2.0.0#shared
ontouml:shared rdf:type owl:NamedIndividual ,
                        ontouml:AggregationKind ;
               rdfs:comment "Indicates that the ontouml:Property has shared aggregation semantics."@en ;
               rdfs:isDefinedBy <https://w3id.org/ontouml/2.0.0> ;
               rdfs:label "shared"@en .


###  https://w3id.org/ontouml/2.0.0#situation
ontouml:situation rdf:type owl:NamedIndividual ,
                           ontouml:ClassStereotype ;
                  rdfs:comment "Can be used to represent certain configurations of entities that can be comprehended as a whole."@en ;
                  rdfs:isDefinedBy <https://w3id.org/ontouml/2.0.0> ;
                  rdfs:label "situation"@en .


###  https://w3id.org/ontouml/2.0.0#situationNature
ontouml:situationNature rdf:type owl:NamedIndividual ,
                                 ontouml:OntologicalNature ;
                        rdfs:comment "Indicates that the restricted type includes situation individuals among its instances."@en ;
                        rdfs:isDefinedBy <https://w3id.org/ontouml/2.0.0> ;
                        rdfs:label "situation nature"@en .


###  https://w3id.org/ontouml/2.0.0#subCollectionOf
ontouml:subCollectionOf rdf:type owl:NamedIndividual ,
                                 ontouml:RelationStereotype ;
                        rdfs:comment "A parthood relation between two collectives."@en ;
                        rdfs:isDefinedBy <https://w3id.org/ontouml/2.0.0> ;
                        rdfs:label "sub collection of"@en ;
                        rdfs:seeAlso "https://ontouml.readthedocs.io/en/latest/relationships/aggregations/subCollectionOf/index.html"^^xsd:anyURI .


###  https://w3id.org/ontouml/2.0.0#subQuantityOf
ontouml:subQuantityOf rdf:type owl:NamedIndividual ,
                               ontouml:RelationStereotype ;
                      rdfs:comment "A parthood relation between two quantities."@en ;
                      rdfs:isDefinedBy <https://w3id.org/ontouml/2.0.0> ;
                      rdfs:label "sub quantity of"@en ;
                      rdfs:seeAlso "https://ontouml.readthedocs.io/en/latest/relationships/aggregations/subQuantityOf/index.html"^^xsd:anyURI .


###  https://w3id.org/ontouml/2.0.0#subkind
ontouml:subkind rdf:type owl:NamedIndividual ,
                         ontouml:ClassStereotype ;
                rdfs:comment "Used to represent rigid specializations of identity providers (Kind, Collective, Quantity, Relator, Mode, and Quantity)."@en ;
                rdfs:isDefinedBy <https://w3id.org/ontouml/2.0.0> ;
                rdfs:label "subkind"@en ;
                rdfs:seeAlso "https://ontouml.readthedocs.io/en/latest/classes/sortals/subkind/index.html"^^xsd:anyURI .


###  https://w3id.org/ontouml/2.0.0#termination
ontouml:termination rdf:type owl:NamedIndividual ,
                             ontouml:RelationStereotype ;
                    rdfs:comment "An individual of the ontouml:RelationStereotype used to assign the corresponding stereotype to a given ontouml:Relation."@en ;
                    rdfs:isDefinedBy <https://w3id.org/ontouml/2.0.0> ;
                    rdfs:label "termination"@en .


###  https://w3id.org/ontouml/2.0.0#triggers
ontouml:triggers rdf:type owl:NamedIndividual ,
                          ontouml:RelationStereotype ;
                 rdfs:comment "An individual of the ontouml:RelationStereotype used to assign the corresponding stereotype to a given ontouml:Relation."@en ;
                 rdfs:isDefinedBy <https://w3id.org/ontouml/2.0.0> ;
                 rdfs:label "triggers"@en .


###  https://w3id.org/ontouml/2.0.0#type
ontouml:type rdf:type owl:NamedIndividual ,
                      ontouml:ClassStereotype ;
             rdfs:comment "The stereotype for high-order types."@en ;
             rdfs:isDefinedBy <https://w3id.org/ontouml/2.0.0> ;
             rdfs:label "type"@en ;
             rdfs:seeAlso <https://doi.org/10.1007/978-3-031-17995-2_2> .


###  https://w3id.org/ontouml/2.0.0#typeNature
ontouml:typeNature rdf:type owl:NamedIndividual ,
                            ontouml:OntologicalNature ;
                   rdfs:comment "Indicates that the restricted type includes type individuals among its instances."@en ;
                   rdfs:isDefinedBy <https://w3id.org/ontouml/2.0.0> ;
                   rdfs:label "type nature"@en .


###  https://www.inf.unibz.it/krdb/
<https://www.inf.unibz.it/krdb/> rdf:type owl:NamedIndividual ,
                                          foaf:Organization ;
                                 foaf:homepage "https://www.inf.unibz.it/krdb/"^^xsd:anyURI ;
                                 foaf:member <https://orcid.org/0000-0003-3385-4769> ;
                                 foaf:name "KRDB Research Centre for Knowledge and Data, Free University of Bozen-Bolzano, Italy" .


###  https://www.utwente.nl/en/eemcs/scs/
<https://www.utwente.nl/en/eemcs/scs/> rdf:type owl:NamedIndividual ,
                                                foaf:Organization ;
                                       foaf:homepage "https://www.utwente.nl/en/eemcs/scs/"^^xsd:anyURI ;
                                       foaf:member <https://orcid.org/0000-0002-5385-5761> ,
                                                   <https://orcid.org/0000-0003-2528-3118> ,
                                                   <https://orcid.org/0000-0003-2736-7817> ;
                                       foaf:name "Semantics, Cybersecurity & Services (SCS), University of Twente, the Netherlands" .


#################################################################
#    Annotations
#################################################################

dct:contributor rdfs:isDefinedBy dct: ;
                rdfs:label "contributor"@en ;
                rdfs:comment "Identifies a foaf:Agent who contributed to the development of the ontouml:NamedElement."@en .


dct:creator rdfs:isDefinedBy dct: ;
            rdfs:comment "Identifies a foaf:Agent who contributed to the creation of the ontouml:NamedElement."@en ;
            rdfs:label "creator"@en .


dct:language rdfs:label "language"@en ;
             rdfs:comment "Determines a language in which the lexical labels of the ontouml:Project are written using strings. This field should use values listed in the IANA Language Sub Tag Registry, such as, \"en\" and \"pt\"."@en ;
             rdfs:isDefinedBy dct: .


dct:license rdfs:label "license"@en ;
            rdfs:isDefinedBy dct: ;
            rdfs:comment "Identifies a legal document under which the ontouml:Project is made available, e.g., \"CC BY 4.0\" <https://creativecommons.org/licenses/by/4.0/>."@en .


dct:publisher rdfs:label "publisher"@en ;
              rdfs:comment "Identifies the foaf:Agent responsible for making the ontouml:Project available. The publisher does not need to have created or contributed to the resource."@en ;
              rdfs:isDefinedBy dct: .


dcat:keyword rdfs:label "keyword"@en ;
             rdfs:comment "Determines the domains (partially) described by the ontouml:Project using a xsd:string or a rdf:langString literal. E.g., the User Feedback Ontology can be described with the keywords \"online user feedback\", \"software engineering\", and \"requirements engineering.\""@en ;
             rdfs:isDefinedBy <http://www.w3.org/ns/dcat> .


dcat:landingPage rdfs:comment "Identifies a web page where one can access the ontouml:Project. E.g., <https://www.model-a-platform.com> is the landing page of the Digital Platform Ontology."@en ;
                 rdfs:isDefinedBy <http://www.w3.org/ns/dcat> ;
                 rdfs:label "landing page"@en .


<https://orcid.org/0000-0002-5385-5761> foaf:name "Tiago Prince Sales" ;
                                        foaf:mbox "t.princesales@utwente.nl" .


<https://orcid.org/0000-0003-2528-3118> foaf:name "Claudenir M. Fonseca" ;
                                        foaf:mbox "c.moraisfonseca@utwente.nl" .


<https://orcid.org/0000-0003-2736-7817> foaf:name "Pedro Paulo Favato Barcelos" ;
                                        foaf:mbox "p.p.favatobarcelos@uwente.nl" .


<https://orcid.org/0000-0003-3385-4769> foaf:mbox "mattia.fumagalli@unibz.it" ;
                                        foaf:name "Mattia Fumagalli" .


ontouml:description rdfs:isDefinedBy <https://w3id.org/ontouml/2.0.0> ;
                    rdfs:label "description"@en ;
                    rdfs:comment "Determines a free-text account of the ontouml:NamedElement using a rdf:langString."@en .


ontouml:name rdfs:label "name"@en ;
             rdfs:isDefinedBy <https://w3id.org/ontouml/2.0.0> ;
             rdfs:comment "Determines the ontouml:name of the ontouml:NamedElement using a rdf:langString."@en .


#################################################################
#    General axioms
#################################################################

[ rdf:type owl:AllDisjointClasses ;
  owl:members ( ontouml:AggregationKind
                ontouml:Cardinality
                ontouml:OntologicalNature
                ontouml:OntoumlElement
                ontouml:Point
                ontouml:Stereotype
              )
] .


[ rdf:type owl:AllDifferent ;
  owl:distinctMembers ( <https://w3id.org/ontouml>
                        ontouml:abstract
                        ontouml:abstractNature
                        ontouml:begin
                        ontouml:bringsAbout
                        ontouml:category
                        ontouml:characterization
                        ontouml:collective
                        ontouml:collectiveNature
                        ontouml:comparative
                        ontouml:componentOf
                        ontouml:composite
                        ontouml:creation
                        ontouml:datatype
                        ontouml:derivation
                        ontouml:end
                        ontouml:enumeration
                        ontouml:event
                        ontouml:eventNature
                        ontouml:externalDependence
                        ontouml:extrinsicModeNature
                        ontouml:functionalComplexNature
                        ontouml:historicalDependence
                        ontouml:historicalRole
                        ontouml:historicalRoleMixin
                        ontouml:instantiation
                        ontouml:intrinsicModeNature
                        ontouml:kind
                        ontouml:manifestation
                        ontouml:material
                        ontouml:mediation
                        ontouml:memberOf
                        ontouml:mixin
                        ontouml:mode
                        ontouml:none
                        ontouml:participation
                        ontouml:participational
                        ontouml:phase
                        ontouml:phaseMixin
                        ontouml:quality
                        ontouml:qualityNature
                        ontouml:quantity
                        ontouml:quantityNature
                        ontouml:relator
                        ontouml:relatorNature
                        ontouml:role
                        ontouml:roleMixin
                        ontouml:shared
                        ontouml:situation
                        ontouml:situationNature
                        ontouml:subCollectionOf
                        ontouml:subQuantityOf
                        ontouml:subkind
                        ontouml:termination
                        ontouml:triggers
                        ontouml:type
                        ontouml:typeNature
                        <https://www.inf.unibz.it/krdb/>
                        <https://www.utwente.nl/en/eemcs/scs/>
                      )
] .


###  Generated by the OWL API (version 4.5.9.2019-02-01T07:24:44Z) https://github.com/owlcs/owlapi
